src/Language/PlutusIR/Semantics/Static/Theorems/Weakening.v
@@ -4,76 +4,9 @@ Require Import PlutusCert.Language.PlutusIR.Semantics.Static.Rules.
 
 Import Coq.Strings.String.
 Local Open Scope string_scope.
-
-Definition inclusion (ctx1 ctx2 : Context) : Prop :=
-  Map.inclusion (fst ctx1) (fst ctx2) /\ Map.inclusion (snd ctx1) (snd ctx2).
-
-Lemma inclusion_emptyContext : forall ctx2,
-    inclusion emptyContext ctx2.
-Proof.
-  intros.
-  unfold inclusion.
-  simpl.
-  destruct ctx2 as [ctx2_T ctx2_K].
-  split; apply inclusion_empty.
-Qed.
-
-Lemma inclusion_extendT : forall (ctx1 ctx2 : Context) (y : binderName) (T : Ty),
-    inclusion ctx1 ctx2 ->
-    inclusion (extendT y T ctx1) (extendT y T ctx2).
-Proof.
-  unfold inclusion.
-  intros.
-  split.
-  - intros.
-    simpl.
-    apply H.
-  - intros. 
-    simpl.
-    unfold lookupT.
-    apply inclusion_update.
-    apply H.
-Qed.
-
-Lemma inclusion_extendK : forall (ctx1 ctx2 : Context) (y : binderTyname) (K : Kind),
-    inclusion ctx1 ctx2 ->
-    inclusion (extendK y K ctx1) (extendK y K ctx2).
-Proof.
-  unfold inclusion.
-  intros.
-  split.
-  - intros.
-    unfold lookupK.
-    apply inclusion_update.
-    apply H.
-  - intros.
-    simpl.
-    apply H.
-Qed.
-
-Lemma inclusion_append : forall (ctx1 ctx2 ctx' : Context),
-    inclusion ctx1 ctx2 ->
-    inclusion (Implementations.append ctx' ctx1) (Implementations.append ctx' ctx2).
-Proof.
-  intros.
-  destruct ctx'.
-  split.
-  - simpl.
-    unfold Map.inclusion.
-    intros.
-    destruct (d x); auto.
-    apply H.
-    assumption.
-  - simpl.
-    unfold Map.inclusion.
-    intros.
-    destruct (g x); auto.
-    apply H.
-    assumption.
-Qed.
       
 Lemma weakening__has_kind : forall Delta Delta' T K,
-    Map.inclusion Delta Delta' ->
+    inclusion Delta Delta' ->
     Delta |-* T : K ->
     Delta' |-* T : K.
 Proof.
@@ -91,206 +24,118 @@ Proof.
 Qed.
 
 
-Definition P_has_type ctx t T : Prop :=
-  forall ctx',
-    inclusion ctx ctx' ->
-    ctx' |-+ t : T.
+Definition P_has_type Delta Gamma t T : Prop :=
+  forall Delta' Gamma',
+    inclusion Delta Delta' ->
+    inclusion Gamma Gamma' ->
+    Delta' ,, Gamma' |-+ t : T.
 
 Definition P_constructor_well_formed Delta c : Prop :=
   forall Delta',
-    Map.inclusion Delta Delta' ->
+    inclusion Delta Delta' ->
     Delta' |-ok_c c.
 
-Definition P_bindings_well_formed_nonrec ctx bs : Prop :=
-  forall ctx',
-    inclusion ctx ctx' ->
-    ctx' |-oks_nr bs.
+Definition P_bindings_well_formed_nonrec Delta Gamma bs : Prop :=
+  forall Delta' Gamma',
+    inclusion Delta Delta' ->
+    inclusion Gamma Gamma' ->
+    Delta' ,, Gamma' |-oks_nr bs.
 
-Definition P_bindings_well_formed_rec ctx bs : Prop :=
-  forall ctx',
-    inclusion ctx ctx' ->
-    ctx' |-oks_r bs.
+Definition P_bindings_well_formed_rec Delta Gamma bs : Prop :=
+  forall Delta' Gamma',
+    inclusion Delta Delta' ->
+    inclusion Gamma Gamma' ->
+    Delta' ,, Gamma' |-oks_r bs.
 
-Definition P_binding_well_formed ctx b : Prop :=
-  forall ctx',
-    inclusion ctx ctx' ->
-    ctx' |-ok b.
+Definition P_binding_well_formed Delta Gamma b : Prop :=
+  forall Delta' Gamma',
+    inclusion Delta Delta' ->
+    inclusion Gamma Gamma' ->
+    Delta' ,, Gamma' |-ok b.
+
+#[export] Hint Unfold
+  P_has_type
+  P_constructor_well_formed
+  P_bindings_well_formed_nonrec
+  P_bindings_well_formed_rec
+  P_binding_well_formed 
+  : core.
 
 Lemma weakening : 
-  (forall ctx t T, ctx |-+ t : T -> P_has_type ctx t T) /\
-  (forall ctx bs, ctx |-oks_nr bs -> P_bindings_well_formed_nonrec ctx bs) /\
-  (forall ctx bs, ctx |-oks_r bs -> P_bindings_well_formed_rec ctx bs) /\
-  (forall ctx b, ctx |-ok b -> P_binding_well_formed ctx b).
-Proof.
+  (forall Delta Gamma t T, Delta ,, Gamma |-+ t : T -> P_has_type Delta Gamma t T) /\
+  (forall Delta Gamma bs, Delta ,, Gamma |-oks_nr bs -> P_bindings_well_formed_nonrec Delta Gamma bs) /\
+  (forall Delta Gamma bs, Delta ,, Gamma |-oks_r bs -> P_bindings_well_formed_rec Delta Gamma bs) /\
+  (forall Delta Gamma b, Delta ,, Gamma |-ok b -> P_binding_well_formed Delta Gamma b).
+Proof with eauto using weakening__has_kind, inclusion_update with typing.
   apply has_type__multind with 
     (P := P_has_type) 
     (P0 := P_constructor_well_formed)
     (P1 := P_bindings_well_formed_nonrec)
     (P2 := P_bindings_well_formed_rec)
     (P3 := P_binding_well_formed).
+  all: intros; autounfold; intros...
   - (* T_Let *)
-    intros. unfold P_has_type. intros.
+    subst.
     eapply T_Let.
     + reflexivity.
-    + apply H1.
-      assumption.
-    + apply H3.
-      subst.
-      apply inclusion_append.
-      assumption.
+    + reflexivity.
+    + apply H2.
+      * assumption.
+      * assumption.
+    + apply H4.
+      * apply inclusion_mupdate.
+        assumption.
+      * apply inclusion_mupdate.
+        assumption.
   - (* T_LetRec *)
-    intros. unfold P_has_type. intros.
+    subst.
     eapply T_LetRec.
     + reflexivity.
-    + apply H1.
-      subst.
-      apply inclusion_append.
-      assumption.
-    + apply H3.
-      subst.
-      apply inclusion_append.
-      assumption.
-  - (* T_Var *)
-    intros. unfold P_has_type. intros.
-    apply T_Var.
-    apply H0.
-    assumption.
-  - (* T_TyAbs *)
-    intros. unfold P_has_type. intros.
-    apply T_TyAbs.
-    apply H0.
-    apply inclusion_extendK.
-    assumption.
-  - (* T_LamAbs *)
-    intros. unfold P_has_type. intros.
-    apply T_LamAbs.
-    + apply H0.
-      apply inclusion_extendT.
-      assumption.
-    + apply weakening__has_kind with (fst ctx).
-      * apply H2.
-      * assumption.
-  - (* T_Apply *)
-    intros. unfold P_has_type. intros.
-    apply T_Apply with T1.
-    + apply H0.
-      assumption.
+    + reflexivity.
     + apply H2.
-      assumption.
-  - (* T_Constant *)
-    intros. unfold P_has_type. intros.
-    apply T_Constant.
-  - (* T_Builtin *)
-    intros. unfold P_has_type. intros.
-    apply T_Builtin.
-  - (* T_TyInst *)
-    intros. unfold P_has_type. intros.
-    apply T_TyInst with (T1 := T1) (X := X) (K2 := K2) (T1' := T1').
-    + apply H0.
-      assumption.
-    + apply weakening__has_kind with (fst ctx).
-      * apply H4. 
-      * assumption.
-    + assumption.
-    + assumption.
-  - (* T_Error *)
-    intros. unfold P_has_type. intros.
-    apply T_Error.
-    apply weakening__has_kind with (fst ctx).
-    + simpl. apply H0.
-    + assumption.
-  - (* T_IWrap *)
-    intros. unfold P_has_type. intros.
-    apply T_IWrap with K S.
-    + assumption.
-    + apply H1.
-      assumption.
-    + apply weakening__has_kind with (fst ctx).
-      * apply H4.
-      * assumption.
-    + apply weakening__has_kind with (fst ctx). 
-      * apply H4.
-      * assumption.
-  - (* T_Unwrap *)
-    intros. unfold P_has_type. intros.
-    apply T_Unwrap with F K T.
-    + apply H0.
-      assumption.
-    + apply weakening__has_kind with (fst ctx).
-      * apply H3. 
-      * assumption.
-    + assumption.
+      * apply inclusion_mupdate.
+        assumption.
+      * apply inclusion_mupdate.
+        assumption.
+    + apply H4.
+      * apply inclusion_mupdate.
+        assumption.
+      * apply inclusion_mupdate.
+        assumption.
   - (* T_ExtBuiltin *)
-    intros. unfold P_has_type. intros.
     eapply T_ExtBuiltin; eauto.
     intros.
     eapply H2; eauto.
-
-  - (* W_Con *)
-    intros. unfold P_constructor_well_formed. intros.
-    eapply W_Con; eauto.
-    intros.
-    apply weakening__has_kind with Delta.
-    + apply H1.
-    + apply H0.
-      assumption.
-  
-  - (* W_NilB_NonRec *)
-    intros. unfold P_bindings_well_formed_nonrec. intros.
-    apply W_NilB_NonRec.
   - (* W_ConsB_NonRec *)
-    intros. unfold P_bindings_well_formed_nonrec. intros.
     apply W_ConsB_NonRec.
     + apply H0.
       assumption.
-    + apply H2.
-      apply inclusion_append.
-      assumption.
-  
-  - (* W_NilB_Rec *)  
-    intros. unfold P_bindings_well_formed_rec. intros.
-    apply W_NilB_Rec.
-  - (* W_ConsB_Rec *)
-    intros. unfold P_bindings_well_formed_rec. intros.
-    apply W_ConsB_Rec.
-    + apply H0.
       assumption.
     + apply H2.
+      apply inclusion_mupdate.
       assumption.
-  
-  - (* W_Term *)
-    intros. unfold P_binding_well_formed. intros.
-    apply W_Term.
-    + apply weakening__has_kind with (fst ctx).
-      * apply H2.
-      * assumption.
-    + apply H1.
+      apply inclusion_mupdate.
       assumption.
-  - (* W_Type *)
-    intros. unfold P_binding_well_formed. intros.
-    apply W_Type.
-    apply weakening__has_kind with (fst ctx).
-    + apply H0.
-    + assumption.
   - (* W_Data *)
-    intros. unfold P_binding_well_formed. intros.
     eapply W_Data.
     + reflexivity.
+    + reflexivity.
     + intros.
-      apply H1.
+      apply H2.
       * assumption.
       * subst.
-        apply inclusion_append.
+        apply inclusion_mupdate.
         assumption.
 Qed.
 
-Lemma weakening_empty : forall ctx t T,
-    emptyContext |-+ t : T ->
-    ctx |-+ t : T.
+Lemma weakening_empty : forall Delta Gamma t T,
+    empty ,, empty |-+ t : T ->
+    Delta ,, Gamma |-+ t : T.
 Proof.
-  intros ctx t T Ht.
+  intros Delta Gamma t T Ht.
   apply weakening in Ht.
   unfold P_has_type in Ht.
   apply Ht.
-  apply inclusion_emptyContext.
+  - apply inclusion_empty.
+  - apply inclusion_empty.
 Qed.
