src/Examples/Timelock/Typing.v
@@ -8,424 +8,267 @@ Open Scope string_scope.
 Definition pir_0_original_shadowfix     := Let (NonRec) (cons (TypeBind (TyVarDecl (TyName (Name ("ByteString") (Unique (0)))) (Kind_Base)) (Ty_Builtin (Some (TypeIn (DefaultUniByteString))))) (nil)) (Let (NonRec) (cons (DatatypeBind (Datatype (TyVarDecl (TyName (Name ("Bool") (Unique (11)))) (Kind_Base)) (nil) (Name ("Bool_match") (Unique (12))) (cons (Constructor (VarDecl (Name ("True") (Unique (13))) (Ty_Var (TyName (Name ("Bool") (Unique (11)))))) (0)) (cons (Constructor (VarDecl (Name ("False") (Unique (14))) (Ty_Var (TyName (Name ("Bool") (Unique (11)))))) (0)) (nil))))) (nil)) (Let (NonRec) (cons (TermBind (Strict) (VarDecl (Name ("verifySignature") (Unique (57))) (Ty_Fun (Ty_Builtin (Some (TypeIn (DefaultUniByteString)))) (Ty_Fun (Ty_Builtin (Some (TypeIn (DefaultUniByteString)))) (Ty_Fun (Ty_Builtin (Some (TypeIn (DefaultUniByteString)))) (Ty_Var (TyName (Name ("Bool") (Unique (11))))))))) (LamAbs (Name ("arg") (Unique (53))) (Ty_Builtin (Some (TypeIn (DefaultUniByteString)))) (LamAbs (Name ("arg") (Unique (54))) (Ty_Builtin (Some (TypeIn (DefaultUniByteString)))) (LamAbs (Name ("arg") (Unique (55))) (Ty_Builtin (Some (TypeIn (DefaultUniByteString)))) (Apply (LamAbs (Name ("b") (Unique (56))) (Ty_Builtin (Some (TypeIn (DefaultUniBool)))) (Apply (Apply (Apply (TyInst (Builtin (IfThenElse)) (Ty_Var (TyName (Name ("Bool") (Unique (11)))))) (Var (Name ("b") (Unique (56))))) (Var (Name ("True") (Unique (13))))) (Var (Name ("False") (Unique (14)))))) (Apply (Apply (Apply (Builtin (VerifySignature)) (Var (Name ("arg") (Unique (53))))) (Var (Name ("arg") (Unique (54))))) (Var (Name ("arg") (Unique (55)))))))))) (nil)) (Let (NonRec) (cons (TypeBind (TyVarDecl (TyName (Name ("String") (Unique (2)))) (Kind_Base)) (Ty_Builtin (Some (TypeIn (DefaultUniString))))) (nil)) (Let (NonRec) (cons (DatatypeBind (Datatype (TyVarDecl (TyName (Name ("Unit") (Unique (60)))) (Kind_Base)) (nil) (Name ("Unit_match") (Unique (61))) (cons (Constructor (VarDecl (Name ("Unit") (Unique (62))) (Ty_Var (TyName (Name ("Unit") (Unique (60)))))) (0)) (nil)))) (nil)) (Let (NonRec) (cons (TermBind (Strict) (VarDecl (Name ("trace") (Unique (70))) (Ty_Fun (Ty_Builtin (Some (TypeIn (DefaultUniString)))) (Ty_Var (TyName (Name ("Unit") (Unique (60))))))) (LamAbs (Name ("arg") (Unique (68))) (Ty_Builtin (Some (TypeIn (DefaultUniString)))) (Apply (LamAbs (Name ("b") (Unique (69))) (Ty_Builtin (Some (TypeIn (DefaultUniUnit)))) (Var (Name ("Unit") (Unique (62))))) (Apply (Builtin (Trace)) (Var (Name ("arg") (Unique (68)))))))) (nil)) (Let (NonRec) (cons (TypeBind (TyVarDecl (TyName (Name ("Integer") (Unique (1)))) (Kind_Base)) (Ty_Builtin (Some (TypeIn (DefaultUniInteger))))) (nil)) (Let (NonRec) (cons (TermBind (Strict) (VarDecl (Name ("takeByteString") (Unique (5))) (Ty_Fun (Ty_Builtin (Some (TypeIn (DefaultUniInteger)))) (Ty_Fun (Ty_Builtin (Some (TypeIn (DefaultUniByteString)))) (Ty_Builtin (Some (TypeIn (DefaultUniByteString))))))) (Builtin (TakeByteString))) (nil)) (Let (NonRec) (cons (TermBind (Strict) (VarDecl (Name ("subtractInteger") (Unique (27))) (Ty_Fun (Ty_Builtin (Some (TypeIn (DefaultUniInteger)))) (Ty_Fun (Ty_Builtin (Some (TypeIn (DefaultUniInteger)))) (Ty_Builtin (Some (TypeIn (DefaultUniInteger))))))) (Builtin (SubtractInteger))) (nil)) (Let (NonRec) (cons (TermBind (Strict) (VarDecl (Name ("sha3_") (Unique (8))) (Ty_Fun (Ty_Builtin (Some (TypeIn (DefaultUniByteString)))) (Ty_Builtin (Some (TypeIn (DefaultUniByteString)))))) (Builtin (SHA3))) (nil)) (Let (NonRec) (cons (TermBind (Strict) (VarDecl (Name ("sha2_") (Unique (7))) (Ty_Fun (Ty_Builtin (Some (TypeIn (DefaultUniByteString)))) (Ty_Builtin (Some (TypeIn (DefaultUniByteString)))))) (Builtin (SHA2))) (nil)) (Let (NonRec) (cons (TermBind (Strict) (VarDecl (Name ("remainderInteger") (Unique (32))) (Ty_Fun (Ty_Builtin (Some (TypeIn (DefaultUniInteger)))) (Ty_Fun (Ty_Builtin (Some (TypeIn (DefaultUniInteger)))) (Ty_Builtin (Some (TypeIn (DefaultUniInteger))))))) (Builtin (RemainderInteger))) (nil)) (Let (NonRec) (cons (TermBind (Strict) (VarDecl (Name ("quotientInteger") (Unique (31))) (Ty_Fun (Ty_Builtin (Some (TypeIn (DefaultUniInteger)))) (Ty_Fun (Ty_Builtin (Some (TypeIn (DefaultUniInteger)))) (Ty_Builtin (Some (TypeIn (DefaultUniInteger))))))) (Builtin (QuotientInteger))) (nil)) (Let (NonRec) (cons (TermBind (Strict) (VarDecl (Name ("multiplyInteger") (Unique (28))) (Ty_Fun (Ty_Builtin (Some (TypeIn (DefaultUniInteger)))) (Ty_Fun (Ty_Builtin (Some (TypeIn (DefaultUniInteger)))) (Ty_Builtin (Some (TypeIn (DefaultUniInteger))))))) (Builtin (MultiplyInteger))) (nil)) (Let (NonRec) (cons (TermBind (Strict) (VarDecl (Name ("modInteger") (Unique (30))) (Ty_Fun (Ty_Builtin (Some (TypeIn (DefaultUniInteger)))) (Ty_Fun (Ty_Builtin (Some (TypeIn (DefaultUniInteger)))) (Ty_Builtin (Some (TypeIn (DefaultUniInteger))))))) (Builtin (ModInteger))) (nil)) (Let (NonRec) (cons (TermBind (Strict) (VarDecl (Name ("lessThanInteger") (Unique (44))) (Ty_Fun (Ty_Builtin (Some (TypeIn (DefaultUniInteger)))) (Ty_Fun (Ty_Builtin (Some (TypeIn (DefaultUniInteger)))) (Ty_Var (TyName (Name ("Bool") (Unique (11)))))))) (LamAbs (Name ("arg") (Unique (41))) (Ty_Builtin (Some (TypeIn (DefaultUniInteger)))) (LamAbs (Name ("arg") (Unique (42))) (Ty_Builtin (Some (TypeIn (DefaultUniInteger)))) (Apply (LamAbs (Name ("b") (Unique (43))) (Ty_Builtin (Some (TypeIn (DefaultUniBool)))) (Apply (Apply (Apply (TyInst (Builtin (IfThenElse)) (Ty_Var (TyName (Name ("Bool") (Unique (11)))))) (Var (Name ("b") (Unique (43))))) (Var (Name ("True") (Unique (13))))) (Var (Name ("False") (Unique (14)))))) (Apply (Apply (Builtin (LessThanInteger)) (Var (Name ("arg") (Unique (41))))) (Var (Name ("arg") (Unique (42))))))))) (nil)) (Let (NonRec) (cons (TermBind (Strict) (VarDecl (Name ("lessThanEqInteger") (Unique (48))) (Ty_Fun (Ty_Builtin (Some (TypeIn (DefaultUniInteger)))) (Ty_Fun (Ty_Builtin (Some (TypeIn (DefaultUniInteger)))) (Ty_Var (TyName (Name ("Bool") (Unique (11)))))))) (LamAbs (Name ("arg") (Unique (45))) (Ty_Builtin (Some (TypeIn (DefaultUniInteger)))) (LamAbs (Name ("arg") (Unique (46))) (Ty_Builtin (Some (TypeIn (DefaultUniInteger)))) (Apply (LamAbs (Name ("b") (Unique (47))) (Ty_Builtin (Some (TypeIn (DefaultUniBool)))) (Apply (Apply (Apply (TyInst (Builtin (IfThenElse)) (Ty_Var (TyName (Name ("Bool") (Unique (11)))))) (Var (Name ("b") (Unique (47))))) (Var (Name ("True") (Unique (13))))) (Var (Name ("False") (Unique (14)))))) (Apply (Apply (Builtin (LessThanEqInteger)) (Var (Name ("arg") (Unique (45))))) (Var (Name ("arg") (Unique (46))))))))) (nil)) (Let (NonRec) (cons (TermBind (Strict) (VarDecl (Name ("lessThanByteString") (Unique (20))) (Ty_Fun (Ty_Builtin (Some (TypeIn (DefaultUniByteString)))) (Ty_Fun (Ty_Builtin (Some (TypeIn (DefaultUniByteString)))) (Ty_Var (TyName (Name ("Bool") (Unique (11)))))))) (LamAbs (Name ("arg") (Unique (17))) (Ty_Builtin (Some (TypeIn (DefaultUniByteString)))) (LamAbs (Name ("arg") (Unique (18))) (Ty_Builtin (Some (TypeIn (DefaultUniByteString)))) (Apply (LamAbs (Name ("b") (Unique (19))) (Ty_Builtin (Some (TypeIn (DefaultUniBool)))) (Apply (Apply (Apply (TyInst (Builtin (IfThenElse)) (Ty_Var (TyName (Name ("Bool") (Unique (11)))))) (Var (Name ("b") (Unique (19))))) (Var (Name ("True") (Unique (13))))) (Var (Name ("False") (Unique (14)))))) (Apply (Apply (Builtin (LtByteString)) (Var (Name ("arg") (Unique (17))))) (Var (Name ("arg") (Unique (18))))))))) (nil)) (Let (NonRec) (cons (TermBind (Strict) (VarDecl (Name ("greaterThanInteger") (Unique (36))) (Ty_Fun (Ty_Builtin (Some (TypeIn (DefaultUniInteger)))) (Ty_Fun (Ty_Builtin (Some (TypeIn (DefaultUniInteger)))) (Ty_Var (TyName (Name ("Bool") (Unique (11)))))))) (LamAbs (Name ("arg") (Unique (33))) (Ty_Builtin (Some (TypeIn (DefaultUniInteger)))) (LamAbs (Name ("arg") (Unique (34))) (Ty_Builtin (Some (TypeIn (DefaultUniInteger)))) (Apply (LamAbs (Name ("b") (Unique (35))) (Ty_Builtin (Some (TypeIn (DefaultUniBool)))) (Apply (Apply (Apply (TyInst (Builtin (IfThenElse)) (Ty_Var (TyName (Name ("Bool") (Unique (11)))))) (Var (Name ("b") (Unique (35))))) (Var (Name ("True") (Unique (13))))) (Var (Name ("False") (Unique (14)))))) (Apply (Apply (Builtin (GreaterThanInteger)) (Var (Name ("arg") (Unique (33))))) (Var (Name ("arg") (Unique (34))))))))) (nil)) (Let (NonRec) (cons (TermBind (Strict) (VarDecl (Name ("greaterThanEqInteger") (Unique (40))) (Ty_Fun (Ty_Builtin (Some (TypeIn (DefaultUniInteger)))) (Ty_Fun (Ty_Builtin (Some (TypeIn (DefaultUniInteger)))) (Ty_Var (TyName (Name ("Bool") (Unique (11)))))))) (LamAbs (Name ("arg") (Unique (37))) (Ty_Builtin (Some (TypeIn (DefaultUniInteger)))) (LamAbs (Name ("arg") (Unique (38))) (Ty_Builtin (Some (TypeIn (DefaultUniInteger)))) (Apply (LamAbs (Name ("b") (Unique (39))) (Ty_Builtin (Some (TypeIn (DefaultUniBool)))) (Apply (Apply (Apply (TyInst (Builtin (IfThenElse)) (Ty_Var (TyName (Name ("Bool") (Unique (11)))))) (Var (Name ("b") (Unique (39))))) (Var (Name ("True") (Unique (13))))) (Var (Name ("False") (Unique (14)))))) (Apply (Apply (Builtin (GreaterThanEqInteger)) (Var (Name ("arg") (Unique (37))))) (Var (Name ("arg") (Unique (38))))))))) (nil)) (Let (NonRec) (cons (TermBind (Strict) (VarDecl (Name ("greaterThanByteString") (Unique (24))) (Ty_Fun (Ty_Builtin (Some (TypeIn (DefaultUniByteString)))) (Ty_Fun (Ty_Builtin (Some (TypeIn (DefaultUniByteString)))) (Ty_Var (TyName (Name ("Bool") (Unique (11)))))))) (LamAbs (Name ("arg") (Unique (21))) (Ty_Builtin (Some (TypeIn (DefaultUniByteString)))) (LamAbs (Name ("arg") (Unique (22))) (Ty_Builtin (Some (TypeIn (DefaultUniByteString)))) (Apply (LamAbs (Name ("b") (Unique (23))) (Ty_Builtin (Some (TypeIn (DefaultUniBool)))) (Apply (Apply (Apply (TyInst (Builtin (IfThenElse)) (Ty_Var (TyName (Name ("Bool") (Unique (11)))))) (Var (Name ("b") (Unique (23))))) (Var (Name ("True") (Unique (13))))) (Var (Name ("False") (Unique (14)))))) (Apply (Apply (Builtin (GtByteString)) (Var (Name ("arg") (Unique (21))))) (Var (Name ("arg") (Unique (22))))))))) (nil)) (Let (NonRec) (cons (TermBind (Strict) (VarDecl (Name ("error") (Unique (64))) (Ty_Forall (TyName (Name ("a") (Unique (63)))) (Kind_Base) (Ty_Fun (Ty_Var (TyName (Name ("Unit") (Unique (60))))) (Ty_Var (TyName (Name ("a") (Unique (63)))))))) (TyAbs (TyName (Name ("e") (Unique (58)))) (Kind_Base) (LamAbs (Name ("thunk") (Unique (59))) (Ty_Var (TyName (Name ("Unit") (Unique (60))))) (Error (Ty_Var (TyName (Name ("e") (Unique (58))))))))) (nil)) (Let (NonRec) (cons (TermBind (Strict) (VarDecl (Name ("equalsInteger") (Unique (52))) (Ty_Fun (Ty_Builtin (Some (TypeIn (DefaultUniInteger)))) (Ty_Fun (Ty_Builtin (Some (TypeIn (DefaultUniInteger)))) (Ty_Var (TyName (Name ("Bool") (Unique (11)))))))) (LamAbs (Name ("arg") (Unique (49))) (Ty_Builtin (Some (TypeIn (DefaultUniInteger)))) (LamAbs (Name ("arg") (Unique (50))) (Ty_Builtin (Some (TypeIn (DefaultUniInteger)))) (Apply (LamAbs (Name ("b") (Unique (51))) (Ty_Builtin (Some (TypeIn (DefaultUniBool)))) (Apply (Apply (Apply (TyInst (Builtin (IfThenElse)) (Ty_Var (TyName (Name ("Bool") (Unique (11)))))) (Var (Name ("b") (Unique (51))))) (Var (Name ("True") (Unique (13))))) (Var (Name ("False") (Unique (14)))))) (Apply (Apply (Builtin (EqInteger)) (Var (Name ("arg") (Unique (49))))) (Var (Name ("arg") (Unique (50))))))))) (nil)) (Let (NonRec) (cons (TermBind (Strict) (VarDecl (Name ("equalsByteString") (Unique (16))) (Ty_Fun (Ty_Builtin (Some (TypeIn (DefaultUniByteString)))) (Ty_Fun (Ty_Builtin (Some (TypeIn (DefaultUniByteString)))) (Ty_Var (TyName (Name ("Bool") (Unique (11)))))))) (LamAbs (Name ("arg") (Unique (9))) (Ty_Builtin (Some (TypeIn (DefaultUniByteString)))) (LamAbs (Name ("arg") (Unique (10))) (Ty_Builtin (Some (TypeIn (DefaultUniByteString)))) (Apply (LamAbs (Name ("b") (Unique (15))) (Ty_Builtin (Some (TypeIn (DefaultUniBool)))) (Apply (Apply (Apply (TyInst (Builtin (IfThenElse)) (Ty_Var (TyName (Name ("Bool") (Unique (11)))))) (Var (Name ("b") (Unique (15))))) (Var (Name ("True") (Unique (13))))) (Var (Name ("False") (Unique (14)))))) (Apply (Apply (Builtin (EqByteString)) (Var (Name ("arg") (Unique (9))))) (Var (Name ("arg") (Unique (10))))))))) (nil)) (Let (NonRec) (cons (TermBind (Strict) (VarDecl (Name ("emptyString") (Unique (66))) (Ty_Builtin (Some (TypeIn (DefaultUniString))))) (Constant (Some (ValueOf (DefaultUniString) (""))))) (nil)) (Let (NonRec) (cons (TermBind (Strict) (VarDecl (Name ("emptyByteString") (Unique (25))) (Ty_Builtin (Some (TypeIn (DefaultUniByteString))))) (Constant (Some (ValueOf (DefaultUniByteString) (""))))) (nil)) (Let (NonRec) (cons (TermBind (Strict) (VarDecl (Name ("dropByteString") (Unique (6))) (Ty_Fun (Ty_Builtin (Some (TypeIn (DefaultUniInteger)))) (Ty_Fun (Ty_Builtin (Some (TypeIn (DefaultUniByteString)))) (Ty_Builtin (Some (TypeIn (DefaultUniByteString))))))) (Builtin (DropByteString))) (nil)) (Let (NonRec) (cons (TermBind (Strict) (VarDecl (Name ("divideInteger") (Unique (29))) (Ty_Fun (Ty_Builtin (Some (TypeIn (DefaultUniInteger)))) (Ty_Fun (Ty_Builtin (Some (TypeIn (DefaultUniInteger)))) (Ty_Builtin (Some (TypeIn (DefaultUniInteger))))))) (Builtin (DivideInteger))) (nil)) (Let (NonRec) (cons (TermBind (Strict) (VarDecl (Name ("concatenate") (Unique (4))) (Ty_Fun (Ty_Builtin (Some (TypeIn (DefaultUniByteString)))) (Ty_Fun (Ty_Builtin (Some (TypeIn (DefaultUniByteString)))) (Ty_Builtin (Some (TypeIn (DefaultUniByteString))))))) (Builtin (Concatenate))) (nil)) (Let (NonRec) (cons (TypeBind (TyVarDecl (TyName (Name ("Char") (Unique (3)))) (Kind_Base)) (Ty_Builtin (Some (TypeIn (DefaultUniChar))))) (nil)) (Let (NonRec) (cons (TermBind (Strict) (VarDecl (Name ("charToString") (Unique (67))) (Ty_Fun (Ty_Builtin (Some (TypeIn (DefaultUniChar)))) (Ty_Builtin (Some (TypeIn (DefaultUniString)))))) (Builtin (CharToString))) (nil)) (Let (NonRec) (cons (TermBind (Strict) (VarDecl (Name ("appendString") (Unique (65))) (Ty_Fun (Ty_Builtin (Some (TypeIn (DefaultUniString)))) (Ty_Fun (Ty_Builtin (Some (TypeIn (DefaultUniString)))) (Ty_Builtin (Some (TypeIn (DefaultUniString))))))) (Builtin (Append))) (nil)) (Let (NonRec) (cons (TermBind (Strict) (VarDecl (Name ("addInteger") (Unique (26))) (Ty_Fun (Ty_Builtin (Some (TypeIn (DefaultUniInteger)))) (Ty_Fun (Ty_Builtin (Some (TypeIn (DefaultUniInteger)))) (Ty_Builtin (Some (TypeIn (DefaultUniInteger))))))) (Builtin (AddInteger))) (nil)) (Let (NonRec) (cons (DatatypeBind (Datatype (TyVarDecl (TyName (Name ("EndDate") (Unique (71)))) (Kind_Base)) (nil) (Name ("EndDate_match") (Unique (72))) (cons (Constructor (VarDecl (Name ("Fixed") (Unique (73))) (Ty_Fun (Ty_Builtin (Some (TypeIn (DefaultUniInteger)))) (Ty_Var (TyName (Name ("EndDate") (Unique (71))))))) (1)) (cons (Constructor (VarDecl (Name ("Never") (Unique (74))) (Ty_Var (TyName (Name ("EndDate") (Unique (71)))))) (0)) (nil))))) (nil)) (LamAbs (Name ("ds1") (Unique (75))) (Ty_Var (TyName (Name ("EndDate") (Unique (71))))) (LamAbs (Name ("ds2") (Unique (76))) (Ty_Builtin (Some (TypeIn (DefaultUniInteger)))) (Let (NonRec) (cons (TermBind (NonStrict) (VarDecl (Name ("keep") (Unique (77))) (Ty_Var (TyName (Name ("Bool") (Unique (11)))))) (Var (Name ("False") (Unique (14))))) (nil)) (Let (NonRec) (cons (TermBind (NonStrict) (VarDecl (Name ("wild") (Unique (78))) (Ty_Var (TyName (Name ("EndDate") (Unique (71)))))) (Var (Name ("ds1") (Unique (75))))) (nil)) (Apply (Apply (Apply (TyInst (Apply (Var (Name ("EndDate_match") (Unique (72)))) (Var (Name ("ds1") (Unique (75))))) (Ty_Fun (Ty_Var (TyName (Name ("Unit") (Unique (60))))) (Ty_Var (TyName (Name ("Bool") (Unique (11))))))) (LamAbs (Name ("n") (Unique (79))) (Ty_Builtin (Some (TypeIn (DefaultUniInteger)))) (LamAbs (Name ("thunk") (Unique (80))) (Ty_Var (TyName (Name ("Unit") (Unique (60))))) (Apply (Apply (Var (Name ("lessThanEqInteger") (Unique (48)))) (Var (Name ("n") (Unique (79))))) (Var (Name ("ds2") (Unique (76)))))))) (LamAbs (Name ("thunk") (Unique (81))) (Ty_Var (TyName (Name ("Unit") (Unique (60))))) (Var (Name ("keep") (Unique (77)))))) (Var (Name ("Unit") (Unique (62)))))))))))))))))))))))))))))))))))))))))).
 
 Example pir_0_original_shadowfix__typable :
-  emptyContext |-+ pir_0_original_shadowfix : (Ty_Fun (Ty_Var "EndDate") (Ty_Fun (Ty_Builtin (Some (TypeIn DefaultUniInteger))) (Ty_Var "Bool"))).
-Proof.
-  eapply T_Let. {
-    reflexivity.
-  }{
-    apply W_ConsB_NonRec.
-    - apply W_Type.
-      apply K_Builtin.
-    - auto with typing.
-  }
-  simpl. eapply T_Let. {
-    reflexivity.
-  }{
-    apply W_ConsB_NonRec.
-    - eapply W_Data.
-      + reflexivity.
-      + intros. simpl.
-        destruct H. {
-          subst.
-          eapply W_Con.
-          + simpl. eauto.
-          + intros.
-            destruct H.
-        }
-        destruct H. {
-          subst.
-          eapply W_Con.
-          + simpl. eauto.
-          + intros.
-            destruct H.
-        }
+  empty ,, empty |-+ pir_0_original_shadowfix : (Ty_Fun (Ty_Var "EndDate") (Ty_Fun (Ty_Builtin (Some (TypeIn DefaultUniInteger))) (Ty_Var "Bool"))).
+Proof with eauto with typing.
+  eapply T_Let... 
+  simpl. eapply T_Let... {
+    apply W_ConsB_NonRec...
+    eapply W_Data...
+    intros. simpl.
+    destruct H. {
+      subst.
+      eapply W_Con.
+      - simpl. eauto.
+      - intros.
         destruct H.
-    - auto with typing.
+      }
+    destruct H. {
+      subst.
+      eapply W_Con.
+      - simpl. eauto.
+      - intros.
+        destruct H.
+    }
+    destruct H.
   }
-  simpl. eapply T_Let. {
-    reflexivity.
-  }{
-    apply W_ConsB_NonRec.
-    - apply W_Term.
-      + constructor. {
-          apply K_Builtin.
-        }
+  simpl. eapply T_Let... {
+    apply W_ConsB_NonRec...
+    apply W_Term...
+    - constructor...
+      constructor... 
+    - constructor. {
         constructor. {
-          apply K_Builtin.
-        }
-        constructor. {
-          apply K_Builtin.
-        }
-        constructor.
-        reflexivity.
-      + constructor. {
           constructor. {
-            constructor. {
-              apply T_Apply with (Ty_Builtin (Some (TypeIn DefaultUniBool))). {
-                apply T_LamAbs. {
+            apply T_Apply with (Ty_Builtin (Some (TypeIn DefaultUniBool))). {
+              apply T_LamAbs. {
+                apply T_Apply with (Ty_Var (TyName (Name "Bool" (Unique 11)))). {
                   apply T_Apply with (Ty_Var (TyName (Name "Bool" (Unique 11)))). {
-                    apply T_Apply with (Ty_Var (TyName (Name "Bool" (Unique 11)))). {
-                      apply T_Apply with (Ty_Builtin (Some (TypeIn DefaultUniBool))). {
-                        apply T_TyInst with 
-                          (T1 := (Ty_Fun (Ty_Builtin (Some (TypeIn DefaultUniBool))) (Ty_Fun (Ty_Var (TyName (Name "a" (Unique 0)))) (Ty_Fun (Ty_Var (TyName (Name "a" (Unique 0)))) (Ty_Var (TyName (Name "a" (Unique 0))))))))
-                          (X := "a")
-                          (K2 := Kind_Base)
-                          (T1' := (Ty_Fun (Ty_Builtin (Some (TypeIn DefaultUniBool)))
-                          (Ty_Fun (Ty_Var (TyName (Name "Bool" (Unique 11))))
-                             (Ty_Fun (Ty_Var (TyName (Name "Bool" (Unique 11))))
-                                (Ty_Var (TyName (Name "Bool" (Unique 11)))))))). {
-                          apply T_Builtin.
-                        }{
-                          auto with typing.
-                        } {
-                          repeat constructor.
-                        }
-                        simpl.
+                    apply T_Apply with (Ty_Builtin (Some (TypeIn DefaultUniBool))). {
+                      apply T_TyInst with 
+                        (T1 := (Ty_Fun (Ty_Builtin (Some (TypeIn DefaultUniBool))) (Ty_Fun (Ty_Var (TyName (Name "a" (Unique 0)))) (Ty_Fun (Ty_Var (TyName (Name "a" (Unique 0)))) (Ty_Var (TyName (Name "a" (Unique 0))))))))
+                        (X := "a")
+                        (K2 := Kind_Base)
+                        (T1' := (Ty_Fun (Ty_Builtin (Some (TypeIn DefaultUniBool)))
+                        (Ty_Fun (Ty_Var (TyName (Name "Bool" (Unique 11))))
+                            (Ty_Fun (Ty_Var (TyName (Name "Bool" (Unique 11))))
+                              (Ty_Var (TyName (Name "Bool" (Unique 11)))))))). {
+                        apply T_Builtin...
+                      }{
                         auto with typing.
+                      } {
+                        repeat constructor.
                       }
+                      simpl.
                       auto with typing.
                     }
                     auto with typing.
                   }
                   auto with typing.
                 }
-                apply K_Builtin.
+                auto with typing.
               }
-              apply T_Apply with (Ty_Builtin (Some (TypeIn DefaultUniByteString))); auto with typing.
-              apply T_Apply with (Ty_Builtin (Some (TypeIn DefaultUniByteString))); auto with typing.
-              apply T_Apply with (Ty_Builtin (Some (TypeIn DefaultUniByteString))); auto with typing.
-              apply T_Builtin.
+              apply K_Builtin...
             }
-            apply K_Builtin.
+            apply T_Apply with (Ty_Builtin (Some (TypeIn DefaultUniByteString))); auto with typing.
+            apply T_Apply with (Ty_Builtin (Some (TypeIn DefaultUniByteString))); auto with typing.
+            apply T_Apply with (Ty_Builtin (Some (TypeIn DefaultUniByteString))); auto with typing.
           }
-          apply K_Builtin.
+          apply K_Builtin...
         }
-        apply K_Builtin.
-    - auto with typing.
+        apply K_Builtin...
+      }
+      apply K_Builtin...
   }
-  simpl. eapply T_Let. {
-    reflexivity.
-  }{
-    apply W_ConsB_NonRec.
-    - apply W_Type.
-      apply K_Builtin.
-    - auto with typing.
-  }
-  simpl. eapply T_Let. {
-    reflexivity.
-  }{
-    apply W_ConsB_NonRec.
-    - eapply W_Data.
-      + reflexivity.
-      + intros. simpl.
-        destruct H. {
-          subst.
-          eapply W_Con.
-          - simpl. eauto.
-          - intros.
-            destruct H.
-        }
+  simpl. eapply T_Let... 
+  simpl. eapply T_Let... {
+    apply W_ConsB_NonRec...
+    eapply W_Data...
+    intros. simpl.
+    destruct H. {
+      subst.
+      eapply W_Con.
+      - simpl. eauto.
+      - intros.
         destruct H.
-    - auto with typing.
+    }
+    destruct H.
   }
-  simpl. eapply T_Let. {
-    reflexivity.
-  }{
-    apply W_ConsB_NonRec.
-    - apply W_Term.
-      + apply K_Fun. {
-          apply K_Builtin.
-        }
-        apply K_Var.
-        reflexivity.
-      + apply T_LamAbs. {
-          apply T_Apply with (Ty_Builtin (Some (TypeIn DefaultUniUnit))). {
-            apply T_LamAbs. {
-              apply T_Var.
-              reflexivity.
-            }
-            apply K_Builtin.
-          }
-          apply T_Apply with (Ty_Builtin (Some (TypeIn DefaultUniString))). {
-            apply T_Builtin.
-          }
+  simpl. eapply T_Let... {
+    apply W_ConsB_NonRec...
+    apply W_Term...
+    apply T_LamAbs. {
+      apply T_Apply with (Ty_Builtin (Some (TypeIn DefaultUniUnit))). {
+        apply T_LamAbs. {
           apply T_Var.
           reflexivity.
         }
-        apply K_Builtin.
-    - auto with typing.
+        apply K_Builtin...
+      }
+      apply T_Apply with (Ty_Builtin (Some (TypeIn DefaultUniString))). {
+        apply T_Builtin...
+      }
+      apply T_Var.
+      reflexivity.
+    }
+    apply K_Builtin...
   }
-  simpl. eapply T_Let. {
-    reflexivity.
-  }{
-    apply W_ConsB_NonRec.
-    - apply W_Type.
-      apply K_Builtin.
-    - auto with typing.
+  simpl. eapply T_Let... 
+  simpl. eapply T_Let... {
+    apply W_ConsB_NonRec...
+    apply W_Term...
+    apply K_Fun...
   }
-  simpl. eapply T_Let. {
-    reflexivity.
-  }{
-    apply W_ConsB_NonRec.
-    - apply W_Term.
-      + apply K_Fun. {
-          apply K_Builtin.
-        }
-        apply K_Fun. {
-          apply K_Builtin.
-        }
-        apply K_Builtin.
-      + apply T_Builtin.
-    - auto with typing.
+  simpl. eapply T_Let... {
+    apply W_ConsB_NonRec...
+    apply W_Term...
+    apply K_Fun...
   }
-  simpl. eapply T_Let. {
-    reflexivity.
-  }{
-    apply W_ConsB_NonRec.
-    - apply W_Term.
-      + apply K_Fun. {
-          apply K_Builtin.
-        }
-        apply K_Fun. {
-          apply K_Builtin.
-        }
-        apply K_Builtin.
-      + apply T_Builtin.
-    - auto with typing.
+  simpl. eapply T_Let... {
+    apply W_ConsB_NonRec...
+    apply W_Term...
   }
-  simpl. eapply T_Let. {
-    reflexivity.
-  }{
-    apply W_ConsB_NonRec.
-    - apply W_Term.
-      + apply K_Fun. {
-          apply K_Builtin.
-        }
-        apply K_Builtin.
-      + apply T_Builtin.
-    - auto with typing.
+  simpl. eapply T_Let... {
+    apply W_ConsB_NonRec...
+    apply W_Term...
   }
-  simpl. eapply T_Let. {
-    reflexivity.
-  }{
-    apply W_ConsB_NonRec.
-    - apply W_Term.
-      + apply K_Fun. {
-          apply K_Builtin.
-        }
-        apply K_Builtin.
-      + apply T_Builtin.
-    - auto with typing.
+  simpl. eapply T_Let... {
+    apply W_ConsB_NonRec...
+    apply W_Term...
+    apply K_Fun...
   }
-  simpl. eapply T_Let. {
-    reflexivity.
-  }{
-    apply W_ConsB_NonRec.
-    - apply W_Term.
-      + apply K_Fun. {
-          apply K_Builtin.
-        }
-        apply K_Fun. {
-          apply K_Builtin.
-        }
-        apply K_Builtin.
-      + apply T_Builtin.
-    - auto with typing.
+  simpl. eapply T_Let... {
+    apply W_ConsB_NonRec...
+    apply W_Term...
+    apply K_Fun... 
   }
-  simpl. eapply T_Let. {
-    reflexivity.
-  }{
-    apply W_ConsB_NonRec.
-    - apply W_Term.
-      + apply K_Fun. {
-          apply K_Builtin.
-        }
-        apply K_Fun. {
-          apply K_Builtin.
-        }
-        apply K_Builtin.
-      + apply T_Builtin.
-    - auto with typing.
+  simpl. eapply T_Let... {
+    apply W_ConsB_NonRec...
+    apply W_Term...
+    apply K_Fun...
   }
-  simpl. eapply T_Let. {
-    reflexivity.
-  }{
-    apply W_ConsB_NonRec.
-    - apply W_Term.
-      + apply K_Fun. {
-          apply K_Builtin.
-        }
-        apply K_Fun. {
-          apply K_Builtin.
-        }
-        apply K_Builtin.
-      + apply T_Builtin.
-    - auto with typing.
+  simpl. eapply T_Let... {
+    apply W_ConsB_NonRec...
+    apply W_Term...
+    apply K_Fun...
   }
-  simpl. eapply T_Let. {
-    reflexivity.
-  }{
-    apply W_ConsB_NonRec.
-    - apply W_Term.
-      + apply K_Fun. {
-          apply K_Builtin.
-        }
-        apply K_Fun. {
-          apply K_Builtin.
-        }
-        apply K_Builtin.
-      + apply T_Builtin.
-    - auto with typing.
-  }
-  simpl. eapply T_Let. {
-    reflexivity.
-  }{
-    apply W_ConsB_NonRec.
-    - apply W_Term.
-      + apply K_Fun. {
-          apply K_Builtin.
-        }
-        apply K_Fun. {
-          apply K_Builtin.
-        }
-        apply K_Var.
-        reflexivity.
-      + apply T_LamAbs. {
-          apply T_LamAbs. {
-            apply T_Apply with (Ty_Builtin (Some (TypeIn DefaultUniBool))). {
-              apply T_LamAbs. {
+  simpl. eapply T_Let... {
+    apply W_ConsB_NonRec...
+    apply W_Term...
+    - apply K_Fun... 
+    - apply T_LamAbs. {
+        apply T_LamAbs. {
+          apply T_Apply with (Ty_Builtin (Some (TypeIn DefaultUniBool))). {
+            apply T_LamAbs. {
+              apply T_Apply with (Ty_Var (TyName (Name "Bool" (Unique 11)))). {
                 apply T_Apply with (Ty_Var (TyName (Name "Bool" (Unique 11)))). {
-                  apply T_Apply with (Ty_Var (TyName (Name "Bool" (Unique 11)))). {
-                    apply T_Apply with (Ty_Builtin (Some (TypeIn DefaultUniBool))). {
-                      apply T_TyInst with 
-                        (T1 := Ty_Fun (Ty_Builtin (Some (TypeIn DefaultUniBool))) (Ty_Fun (Ty_Var (TyName (Name "a" (Unique 0)))) (Ty_Fun (Ty_Var (TyName (Name "a" (Unique 0)))) (Ty_Var (TyName (Name "a" (Unique 0)))))))
-                        (X := "a")
-                        (K2 := Kind_Base)
-                        (T1' := (Ty_Fun (Ty_Builtin (Some (TypeIn DefaultUniBool)))
-                        (Ty_Fun (Ty_Var (TyName (Name "Bool" (Unique 11))))
-                           (Ty_Fun (Ty_Var (TyName (Name "Bool" (Unique 11))))
-                              (Ty_Var (TyName (Name "Bool" (Unique 11)))))))). {
-                        apply T_Builtin.
-                      }{
-                        auto with typing.
-                      } {
-                        repeat constructor.
-                      }
+                  apply T_Apply with (Ty_Builtin (Some (TypeIn DefaultUniBool))). {
+                    apply T_TyInst with 
+                      (T1 := Ty_Fun (Ty_Builtin (Some (TypeIn DefaultUniBool))) (Ty_Fun (Ty_Var (TyName (Name "a" (Unique 0)))) (Ty_Fun (Ty_Var (TyName (Name "a" (Unique 0)))) (Ty_Var (TyName (Name "a" (Unique 0)))))))
+                      (X := "a")
+                      (K2 := Kind_Base)
+                      (T1' := (Ty_Fun (Ty_Builtin (Some (TypeIn DefaultUniBool)))
+                      (Ty_Fun (Ty_Var (TyName (Name "Bool" (Unique 11))))
+                          (Ty_Fun (Ty_Var (TyName (Name "Bool" (Unique 11))))
+                            (Ty_Var (TyName (Name "Bool" (Unique 11)))))))). {
+                      apply T_Builtin...
+                    }{
                       auto with typing.
+                    } {
+                      repeat constructor.
                     }
                     auto with typing.
                   }
                   auto with typing.
                 }
                 auto with typing.
-              }
-              apply K_Builtin.
-            }
-            apply T_Apply with (Ty_Builtin (Some (TypeIn DefaultUniInteger))). {
-              apply T_Apply with (Ty_Builtin (Some (TypeIn DefaultUniInteger))). {
-                apply T_Builtin.
               }
               auto with typing.
             }
+            apply K_Builtin...
+          }
+          apply T_Apply with (Ty_Builtin (Some (TypeIn DefaultUniInteger))). {
+            apply T_Apply with (Ty_Builtin (Some (TypeIn DefaultUniInteger))). {
+              apply T_Builtin...
+            }
             auto with typing.
           }
-          apply K_Builtin.
+          auto with typing.
         }
-        apply K_Builtin.
-    - auto with typing.
+        apply K_Builtin...
+      }
+      apply K_Builtin...
   }
-  simpl. eapply T_Let. {
-    reflexivity.
-  }{
-    apply W_ConsB_NonRec.
-    - apply W_Term.
-      + apply K_Fun. {
-          apply K_Builtin.
-        }
-        apply K_Fun. {
-          apply K_Builtin.
-        }
-        apply K_Var.
-        reflexivity.
-      + apply T_LamAbs. {
-          apply T_LamAbs. {
-            apply T_Apply with (Ty_Builtin (Some (TypeIn DefaultUniBool))). {
-              apply T_LamAbs. {
+  simpl. eapply T_Let... {
+    apply W_ConsB_NonRec...
+    apply W_Term...
+    - apply K_Fun...
+    - apply T_LamAbs. {
+        apply T_LamAbs. {
+          apply T_Apply with (Ty_Builtin (Some (TypeIn DefaultUniBool))). {
+            apply T_LamAbs. {
+              apply T_Apply with (Ty_Var (TyName (Name "Bool" (Unique 11)))). {
                 apply T_Apply with (Ty_Var (TyName (Name "Bool" (Unique 11)))). {
-                  apply T_Apply with (Ty_Var (TyName (Name "Bool" (Unique 11)))). {
-                    apply T_Apply with (Ty_Builtin (Some (TypeIn DefaultUniBool))). {
-                      apply T_TyInst with 
-                        (T1 := Ty_Fun (Ty_Builtin (Some (TypeIn DefaultUniBool))) (Ty_Fun (Ty_Var (TyName (Name "a" (Unique 0)))) (Ty_Fun (Ty_Var (TyName (Name "a" (Unique 0)))) (Ty_Var (TyName (Name "a" (Unique 0)))))))
-                        (X := "a")
-                        (K2 := Kind_Base)
-                        (T1' := (Ty_Fun (Ty_Builtin (Some (TypeIn DefaultUniBool)))
+                  apply T_Apply with (Ty_Builtin (Some (TypeIn DefaultUniBool))). {
+                    apply T_TyInst with 
+                      (T1 := Ty_Fun (Ty_Builtin (Some (TypeIn DefaultUniBool))) (Ty_Fun (Ty_Var (TyName (Name "a" (Unique 0)))) (Ty_Fun (Ty_Var (TyName (Name "a" (Unique 0)))) (Ty_Var (TyName (Name "a" (Unique 0)))))))
+                      (X := "a")
+                      (K2 := Kind_Base)
+                      (T1' := (Ty_Fun (Ty_Builtin (Some (TypeIn DefaultUniBool)))
+                      (Ty_Fun (Ty_Var (TyName (Name "Bool" (Unique 11))))
                         (Ty_Fun (Ty_Var (TyName (Name "Bool" (Unique 11))))
-                           (Ty_Fun (Ty_Var (TyName (Name "Bool" (Unique 11))))
-                              (Ty_Var (TyName (Name "Bool" (Unique 11)))))))). {
-                        apply T_Builtin.
-                      }{
-                        auto with typing.
-                      } {
-                        repeat constructor.
-                      }
+                            (Ty_Var (TyName (Name "Bool" (Unique 11)))))))). {
+                      apply T_Builtin...
+                    }{
                       auto with typing.
+                    } {
+                      repeat constructor.
                     }
                     auto with typing.
                   }
                   auto with typing.
                 }
                 auto with typing.
-              }
-              apply K_Builtin.
-            }
-            apply T_Apply with (Ty_Builtin (Some (TypeIn DefaultUniInteger))). {
-              apply T_Apply with (Ty_Builtin (Some (TypeIn DefaultUniInteger))). {
-                apply T_Builtin.
               }
               auto with typing.
             }
+            apply K_Builtin...
+          }
+          apply T_Apply with (Ty_Builtin (Some (TypeIn DefaultUniInteger))). {
+            apply T_Apply with (Ty_Builtin (Some (TypeIn DefaultUniInteger))). {
+              apply T_Builtin...
+            }
             auto with typing.
           }
-          apply K_Builtin.
+          auto with typing.
         }
-        apply K_Builtin.
-    - auto with typing.
+        apply K_Builtin...
+      }
+      apply K_Builtin...
   }
-  simpl. eapply T_Let. {
-    reflexivity.
-  }{
-    apply W_ConsB_NonRec.
-    - apply W_Term.
-      + apply K_Fun. {
-          apply K_Builtin.
-        }
-        apply K_Fun. {
-          apply K_Builtin.
-        }
-        apply K_Var.
-        reflexivity.
-      + apply T_LamAbs. {
-          apply T_LamAbs. {
-            apply T_Apply with (Ty_Builtin (Some (TypeIn DefaultUniBool))). {
-              apply T_LamAbs. {
+  simpl. eapply T_Let... {
+    apply W_ConsB_NonRec...
+    apply W_Term...
+    - apply K_Fun... 
+    - apply T_LamAbs. {
+        apply T_LamAbs. {
+          apply T_Apply with (Ty_Builtin (Some (TypeIn DefaultUniBool))). {
+            apply T_LamAbs. {
+              apply T_Apply with (Ty_Var (TyName (Name "Bool" (Unique 11)))). {
                 apply T_Apply with (Ty_Var (TyName (Name "Bool" (Unique 11)))). {
-                  apply T_Apply with (Ty_Var (TyName (Name "Bool" (Unique 11)))). {
-                    apply T_Apply with (Ty_Builtin (Some (TypeIn DefaultUniBool))). {
-                      apply T_TyInst with 
-                        (T1 := Ty_Fun (Ty_Builtin (Some (TypeIn DefaultUniBool))) (Ty_Fun (Ty_Var (TyName (Name "a" (Unique 0)))) (Ty_Fun (Ty_Var (TyName (Name "a" (Unique 0)))) (Ty_Var (TyName (Name "a" (Unique 0)))))))
-                        (X := "a")
-                        (K2 := Kind_Base)
-                        (T1' := (Ty_Fun (Ty_Builtin (Some (TypeIn DefaultUniBool)))
-                        (Ty_Fun (Ty_Var (TyName (Name "Bool" (Unique 11))))
-                           (Ty_Fun (Ty_Var (TyName (Name "Bool" (Unique 11))))
-                              (Ty_Var (TyName (Name "Bool" (Unique 11)))))))). {
-                        apply T_Builtin.
-                      }{
-                        auto with typing.
-                      } {
-                        repeat constructor.
-                      }
+                  apply T_Apply with (Ty_Builtin (Some (TypeIn DefaultUniBool))). {
+                    apply T_TyInst with 
+                      (T1 := Ty_Fun (Ty_Builtin (Some (TypeIn DefaultUniBool))) (Ty_Fun (Ty_Var (TyName (Name "a" (Unique 0)))) (Ty_Fun (Ty_Var (TyName (Name "a" (Unique 0)))) (Ty_Var (TyName (Name "a" (Unique 0)))))))
+                      (X := "a")
+                      (K2 := Kind_Base)
+                      (T1' := (Ty_Fun (Ty_Builtin (Some (TypeIn DefaultUniBool)))
+                      (Ty_Fun (Ty_Var (TyName (Name "Bool" (Unique 11))))
+                          (Ty_Fun (Ty_Var (TyName (Name "Bool" (Unique 11))))
+                            (Ty_Var (TyName (Name "Bool" (Unique 11)))))))). {
+                      apply T_Builtin...
+                    }{
                       auto with typing.
+                    } {
+                      repeat constructor.
                     }
                     auto with typing.
                   }
@@ -433,56 +276,46 @@ Proof.
                 }
                 auto with typing.
               }
-              apply K_Builtin.
+              auto with typing.
             }
+            apply K_Builtin...
+          }
+          apply T_Apply with (Ty_Builtin (Some (TypeIn DefaultUniByteString))). {
             apply T_Apply with (Ty_Builtin (Some (TypeIn DefaultUniByteString))). {
-              apply T_Apply with (Ty_Builtin (Some (TypeIn DefaultUniByteString))). {
-                apply T_Builtin.
-              }
-              auto with typing.
+              apply T_Builtin...
             }
             auto with typing.
           }
-          apply K_Builtin.
+          auto with typing.
         }
-        apply K_Builtin.
-    - auto with typing.
+        apply K_Builtin...
+      }
+      apply K_Builtin...
   }
-  simpl. eapply T_Let. {
-    reflexivity.
-  }{
-    apply W_ConsB_NonRec.
-    - apply W_Term.
-      + apply K_Fun. {
-          apply K_Builtin.
-        }
-        apply K_Fun. {
-          apply K_Builtin.
-        }
-        apply K_Var.
-        reflexivity.
-      + apply T_LamAbs. {
-          apply T_LamAbs. {
-            apply T_Apply with (Ty_Builtin (Some (TypeIn DefaultUniBool))). {
-              apply T_LamAbs. {
+  simpl. eapply T_Let... {
+    apply W_ConsB_NonRec...
+    apply W_Term...
+    - apply K_Fun... 
+    - apply T_LamAbs. {
+        apply T_LamAbs. {
+          apply T_Apply with (Ty_Builtin (Some (TypeIn DefaultUniBool))). {
+            apply T_LamAbs. {
+              apply T_Apply with (Ty_Var (TyName (Name "Bool" (Unique 11)))). {
                 apply T_Apply with (Ty_Var (TyName (Name "Bool" (Unique 11)))). {
-                  apply T_Apply with (Ty_Var (TyName (Name "Bool" (Unique 11)))). {
-                    apply T_Apply with (Ty_Builtin (Some (TypeIn DefaultUniBool))). {
-                      apply T_TyInst with 
-                        (T1 := Ty_Fun (Ty_Builtin (Some (TypeIn DefaultUniBool))) (Ty_Fun (Ty_Var (TyName (Name "a" (Unique 0)))) (Ty_Fun (Ty_Var (TyName (Name "a" (Unique 0)))) (Ty_Var (TyName (Name "a" (Unique 0)))))))
-                        (X := "a")
-                        (K2 := Kind_Base)
-                        (T1' := (Ty_Fun (Ty_Builtin (Some (TypeIn DefaultUniBool)))
-                        (Ty_Fun (Ty_Var (TyName (Name "Bool" (Unique 11))))
-                           (Ty_Fun (Ty_Var (TyName (Name "Bool" (Unique 11))))
-                              (Ty_Var (TyName (Name "Bool" (Unique 11)))))))). {
-                        apply T_Builtin.
-                      }{
-                        auto with typing.
-                      } {
-                        repeat constructor.
-                      }
+                  apply T_Apply with (Ty_Builtin (Some (TypeIn DefaultUniBool))). {
+                    apply T_TyInst with 
+                      (T1 := Ty_Fun (Ty_Builtin (Some (TypeIn DefaultUniBool))) (Ty_Fun (Ty_Var (TyName (Name "a" (Unique 0)))) (Ty_Fun (Ty_Var (TyName (Name "a" (Unique 0)))) (Ty_Var (TyName (Name "a" (Unique 0)))))))
+                      (X := "a")
+                      (K2 := Kind_Base)
+                      (T1' := (Ty_Fun (Ty_Builtin (Some (TypeIn DefaultUniBool)))
+                      (Ty_Fun (Ty_Var (TyName (Name "Bool" (Unique 11))))
+                          (Ty_Fun (Ty_Var (TyName (Name "Bool" (Unique 11))))
+                            (Ty_Var (TyName (Name "Bool" (Unique 11)))))))). {
+                      apply T_Builtin...
+                    }{
                       auto with typing.
+                    } {
+                      repeat constructor.
                     }
                     auto with typing.
                   }
@@ -490,56 +323,46 @@ Proof.
                 }
                 auto with typing.
               }
-              apply K_Builtin.
+              auto with typing.
             }
+            apply K_Builtin...
+          }
+          apply T_Apply with (Ty_Builtin (Some (TypeIn DefaultUniInteger))). {
             apply T_Apply with (Ty_Builtin (Some (TypeIn DefaultUniInteger))). {
-              apply T_Apply with (Ty_Builtin (Some (TypeIn DefaultUniInteger))). {
-                apply T_Builtin.
-              }
-              auto with typing.
+              apply T_Builtin...
             }
             auto with typing.
           }
-          apply K_Builtin.
+          auto with typing.
         }
-        apply K_Builtin.
-    - auto with typing.
+        apply K_Builtin...
+      }
+      apply K_Builtin...
   }
-  simpl. eapply T_Let. {
-    reflexivity.
-  }{
-    apply W_ConsB_NonRec.
-    - apply W_Term.
-      + apply K_Fun. {
-          apply K_Builtin.
-        }
-        apply K_Fun. {
-          apply K_Builtin.
-        }
-        apply K_Var.
-        reflexivity.
-      + apply T_LamAbs. {
-          apply T_LamAbs. {
-            apply T_Apply with (Ty_Builtin (Some (TypeIn DefaultUniBool))). {
-              apply T_LamAbs. {
+  simpl. eapply T_Let... {
+    apply W_ConsB_NonRec...
+    apply W_Term...
+    - apply K_Fun... 
+    - apply T_LamAbs. {
+        apply T_LamAbs. {
+          apply T_Apply with (Ty_Builtin (Some (TypeIn DefaultUniBool))). {
+            apply T_LamAbs. {
+              apply T_Apply with (Ty_Var (TyName (Name "Bool" (Unique 11)))). {
                 apply T_Apply with (Ty_Var (TyName (Name "Bool" (Unique 11)))). {
-                  apply T_Apply with (Ty_Var (TyName (Name "Bool" (Unique 11)))). {
-                    apply T_Apply with (Ty_Builtin (Some (TypeIn DefaultUniBool))). {
-                      apply T_TyInst with 
-                        (T1 := Ty_Fun (Ty_Builtin (Some (TypeIn DefaultUniBool))) (Ty_Fun (Ty_Var (TyName (Name "a" (Unique 0)))) (Ty_Fun (Ty_Var (TyName (Name "a" (Unique 0)))) (Ty_Var (TyName (Name "a" (Unique 0)))))))
-                        (X := "a")
-                        (K2 := Kind_Base)
-                        (T1' := (Ty_Fun (Ty_Builtin (Some (TypeIn DefaultUniBool)))
-                        (Ty_Fun (Ty_Var (TyName (Name "Bool" (Unique 11))))
-                           (Ty_Fun (Ty_Var (TyName (Name "Bool" (Unique 11))))
-                              (Ty_Var (TyName (Name "Bool" (Unique 11)))))))). {
-                        apply T_Builtin.
-                      }{
-                        auto with typing.
-                      } {
-                        repeat constructor.
-                      }
+                  apply T_Apply with (Ty_Builtin (Some (TypeIn DefaultUniBool))). {
+                    apply T_TyInst with 
+                      (T1 := Ty_Fun (Ty_Builtin (Some (TypeIn DefaultUniBool))) (Ty_Fun (Ty_Var (TyName (Name "a" (Unique 0)))) (Ty_Fun (Ty_Var (TyName (Name "a" (Unique 0)))) (Ty_Var (TyName (Name "a" (Unique 0)))))))
+                      (X := "a")
+                      (K2 := Kind_Base)
+                      (T1' := (Ty_Fun (Ty_Builtin (Some (TypeIn DefaultUniBool)))
+                      (Ty_Fun (Ty_Var (TyName (Name "Bool" (Unique 11))))
+                          (Ty_Fun (Ty_Var (TyName (Name "Bool" (Unique 11))))
+                            (Ty_Var (TyName (Name "Bool" (Unique 11)))))))). {
+                      apply T_Builtin...
+                    }{
                       auto with typing.
+                    } {
+                      repeat constructor.
                     }
                     auto with typing.
                   }
@@ -547,56 +370,46 @@ Proof.
                 }
                 auto with typing.
               }
-              apply K_Builtin.
+              auto with typing.
             }
+            apply K_Builtin...
+          }
+          apply T_Apply with (Ty_Builtin (Some (TypeIn DefaultUniInteger))). {
             apply T_Apply with (Ty_Builtin (Some (TypeIn DefaultUniInteger))). {
-              apply T_Apply with (Ty_Builtin (Some (TypeIn DefaultUniInteger))). {
-                apply T_Builtin.
-              }
-              auto with typing.
+              apply T_Builtin...
             }
             auto with typing.
           }
-          apply K_Builtin.
+          auto with typing.
         }
-        apply K_Builtin.
-    - auto with typing.
+        apply K_Builtin...
+      }
+      apply K_Builtin...
   }
-  simpl. eapply T_Let. {
-    reflexivity.
-  }{
-    apply W_ConsB_NonRec.
-    - apply W_Term.
-      + apply K_Fun. {
-          apply K_Builtin.
-        }
-        apply K_Fun. {
-          apply K_Builtin.
-        }
-        apply K_Var.
-        reflexivity.
-      + apply T_LamAbs. {
-          apply T_LamAbs. {
-            apply T_Apply with (Ty_Builtin (Some (TypeIn DefaultUniBool))). {
-              apply T_LamAbs. {
+  simpl. eapply T_Let... {
+    apply W_ConsB_NonRec...
+    apply W_Term...
+    - apply K_Fun... 
+    - apply T_LamAbs. {
+        apply T_LamAbs. {
+          apply T_Apply with (Ty_Builtin (Some (TypeIn DefaultUniBool))). {
+            apply T_LamAbs. {
+              apply T_Apply with (Ty_Var (TyName (Name "Bool" (Unique 11)))). {
                 apply T_Apply with (Ty_Var (TyName (Name "Bool" (Unique 11)))). {
-                  apply T_Apply with (Ty_Var (TyName (Name "Bool" (Unique 11)))). {
-                    apply T_Apply with (Ty_Builtin (Some (TypeIn DefaultUniBool))). {
-                      apply T_TyInst with 
-                        (T1 := Ty_Fun (Ty_Builtin (Some (TypeIn DefaultUniBool))) (Ty_Fun (Ty_Var (TyName (Name "a" (Unique 0)))) (Ty_Fun (Ty_Var (TyName (Name "a" (Unique 0)))) (Ty_Var (TyName (Name "a" (Unique 0)))))))
-                        (X := "a")
-                        (K2 := Kind_Base)
-                        (T1' := (Ty_Fun (Ty_Builtin (Some (TypeIn DefaultUniBool)))
-                        (Ty_Fun (Ty_Var (TyName (Name "Bool" (Unique 11))))
-                           (Ty_Fun (Ty_Var (TyName (Name "Bool" (Unique 11))))
-                              (Ty_Var (TyName (Name "Bool" (Unique 11)))))))). {
-                        apply T_Builtin.
-                      }{
-                        auto with typing.
-                      } {
-                        repeat constructor.
-                      }
+                  apply T_Apply with (Ty_Builtin (Some (TypeIn DefaultUniBool))). {
+                    apply T_TyInst with 
+                      (T1 := Ty_Fun (Ty_Builtin (Some (TypeIn DefaultUniBool))) (Ty_Fun (Ty_Var (TyName (Name "a" (Unique 0)))) (Ty_Fun (Ty_Var (TyName (Name "a" (Unique 0)))) (Ty_Var (TyName (Name "a" (Unique 0)))))))
+                      (X := "a")
+                      (K2 := Kind_Base)
+                      (T1' := (Ty_Fun (Ty_Builtin (Some (TypeIn DefaultUniBool)))
+                      (Ty_Fun (Ty_Var (TyName (Name "Bool" (Unique 11))))
+                          (Ty_Fun (Ty_Var (TyName (Name "Bool" (Unique 11))))
+                            (Ty_Var (TyName (Name "Bool" (Unique 11)))))))). {
+                      apply T_Builtin...
+                    }{
                       auto with typing.
+                    } {
+                      repeat constructor.
                     }
                     auto with typing.
                   }
@@ -604,71 +417,51 @@ Proof.
                 }
                 auto with typing.
               }
-              apply K_Builtin.
+              auto with typing.
             }
+            apply K_Builtin...
+          }
+          apply T_Apply with (Ty_Builtin (Some (TypeIn DefaultUniByteString))). {
             apply T_Apply with (Ty_Builtin (Some (TypeIn DefaultUniByteString))). {
-              apply T_Apply with (Ty_Builtin (Some (TypeIn DefaultUniByteString))). {
-                apply T_Builtin.
-              }
-              auto with typing.
+              apply T_Builtin...
             }
             auto with typing.
           }
-          apply K_Builtin.
+          auto with typing.
         }
-        apply K_Builtin.
-    - auto with typing.
+        apply K_Builtin...
+      }
+      apply K_Builtin...
   }
-  simpl. eapply T_Let. {
-    reflexivity.
-  }{
-    apply W_ConsB_NonRec.
-    - apply W_Term.
-      + apply K_Forall.
-        apply K_Fun. {
-          apply K_Var.
-          reflexivity.
-        }
-        apply K_Var.
-        reflexivity.
-      + (* TODO: alpha-equivalence *) Axiom skip : forall P, P. apply skip.
-    - auto with typing.
+  simpl. eapply T_Let... {
+    apply W_ConsB_NonRec...
+    apply W_Term...
+    (* TODO: alpha-equivalence *) Axiom skip : forall P, P. apply skip.
   }
-  simpl. eapply T_Let. {
-    reflexivity.
-  }{
-    apply W_ConsB_NonRec.
-    - apply W_Term.
-      + apply K_Fun. {
-          apply K_Builtin.
-        }
-        apply K_Fun. {
-          apply K_Builtin.
-        }
-        apply K_Var.
-        reflexivity.
-      + apply T_LamAbs. {
-          apply T_LamAbs. {
-            apply T_Apply with (Ty_Builtin (Some (TypeIn DefaultUniBool))). {
-              apply T_LamAbs. {
+  simpl. eapply T_Let... {
+    apply W_ConsB_NonRec...
+    apply W_Term...
+    - apply K_Fun...
+    - apply T_LamAbs. {
+        apply T_LamAbs. {
+          apply T_Apply with (Ty_Builtin (Some (TypeIn DefaultUniBool))). {
+            apply T_LamAbs. {
+              apply T_Apply with (Ty_Var (TyName (Name "Bool" (Unique 11)))). {
                 apply T_Apply with (Ty_Var (TyName (Name "Bool" (Unique 11)))). {
-                  apply T_Apply with (Ty_Var (TyName (Name "Bool" (Unique 11)))). {
-                    apply T_Apply with (Ty_Builtin (Some (TypeIn DefaultUniBool))). {
-                      apply T_TyInst with 
-                        (T1 := Ty_Fun (Ty_Builtin (Some (TypeIn DefaultUniBool))) (Ty_Fun (Ty_Var (TyName (Name "a" (Unique 0)))) (Ty_Fun (Ty_Var (TyName (Name "a" (Unique 0)))) (Ty_Var (TyName (Name "a" (Unique 0)))))))
-                        (X := "a")
-                        (K2 := Kind_Base)
-                        (T1' := (Ty_Fun (Ty_Builtin (Some (TypeIn DefaultUniBool)))
-                        (Ty_Fun (Ty_Var (TyName (Name "Bool" (Unique 11))))
-                           (Ty_Fun (Ty_Var (TyName (Name "Bool" (Unique 11))))
-                              (Ty_Var (TyName (Name "Bool" (Unique 11)))))))). {
-                        apply T_Builtin.
-                      }{
-                        auto with typing.
-                      } {
-                        repeat constructor.
-                      }
+                  apply T_Apply with (Ty_Builtin (Some (TypeIn DefaultUniBool))). {
+                    apply T_TyInst with 
+                      (T1 := Ty_Fun (Ty_Builtin (Some (TypeIn DefaultUniBool))) (Ty_Fun (Ty_Var (TyName (Name "a" (Unique 0)))) (Ty_Fun (Ty_Var (TyName (Name "a" (Unique 0)))) (Ty_Var (TyName (Name "a" (Unique 0)))))))
+                      (X := "a")
+                      (K2 := Kind_Base)
+                      (T1' := (Ty_Fun (Ty_Builtin (Some (TypeIn DefaultUniBool)))
+                      (Ty_Fun (Ty_Var (TyName (Name "Bool" (Unique 11))))
+                          (Ty_Fun (Ty_Var (TyName (Name "Bool" (Unique 11))))
+                            (Ty_Var (TyName (Name "Bool" (Unique 11)))))))). {
+                      apply T_Builtin...
+                    }{
                       auto with typing.
+                    } {
+                      repeat constructor.
                     }
                     auto with typing.
                   }
@@ -676,56 +469,46 @@ Proof.
                 }
                 auto with typing.
               }
-              apply K_Builtin.
+              auto with typing.
             }
+            apply K_Builtin...
+          }
+          apply T_Apply with (Ty_Builtin (Some (TypeIn DefaultUniInteger))). {
             apply T_Apply with (Ty_Builtin (Some (TypeIn DefaultUniInteger))). {
-              apply T_Apply with (Ty_Builtin (Some (TypeIn DefaultUniInteger))). {
-                apply T_Builtin.
-              }
-              auto with typing.
+              apply T_Builtin...
             }
             auto with typing.
           }
-          apply K_Builtin.
+          auto with typing.
         }
-        apply K_Builtin.
-    - auto with typing.
+        apply K_Builtin...
+      }
+      apply K_Builtin...
   }
-  simpl. eapply T_Let. {
-    reflexivity.
-  }{
-    apply W_ConsB_NonRec.
-    - apply W_Term.
-      + apply K_Fun. {
-          apply K_Builtin.
-        }
-        apply K_Fun. {
-          apply K_Builtin.
-        }
-        apply K_Var.
-        reflexivity.
-      + apply T_LamAbs. {
-          apply T_LamAbs. {
-            apply T_Apply with (Ty_Builtin (Some (TypeIn DefaultUniBool))). {
-              apply T_LamAbs. {
+  simpl. eapply T_Let... {
+    apply W_ConsB_NonRec...
+    apply W_Term...
+    - apply K_Fun... 
+    - apply T_LamAbs. {
+        apply T_LamAbs. {
+          apply T_Apply with (Ty_Builtin (Some (TypeIn DefaultUniBool))). {
+            apply T_LamAbs. {
+              apply T_Apply with (Ty_Var (TyName (Name "Bool" (Unique 11)))). {
                 apply T_Apply with (Ty_Var (TyName (Name "Bool" (Unique 11)))). {
-                  apply T_Apply with (Ty_Var (TyName (Name "Bool" (Unique 11)))). {
-                    apply T_Apply with (Ty_Builtin (Some (TypeIn DefaultUniBool))). {
-                      apply T_TyInst with 
-                        (T1 := Ty_Fun (Ty_Builtin (Some (TypeIn DefaultUniBool))) (Ty_Fun (Ty_Var (TyName (Name "a" (Unique 0)))) (Ty_Fun (Ty_Var (TyName (Name "a" (Unique 0)))) (Ty_Var (TyName (Name "a" (Unique 0)))))))
-                        (X := "a")
-                        (K2 := Kind_Base)
-                        (T1' := (Ty_Fun (Ty_Builtin (Some (TypeIn DefaultUniBool)))
-                        (Ty_Fun (Ty_Var (TyName (Name "Bool" (Unique 11))))
-                           (Ty_Fun (Ty_Var (TyName (Name "Bool" (Unique 11))))
-                              (Ty_Var (TyName (Name "Bool" (Unique 11)))))))). {
-                        apply T_Builtin.
-                      }{
-                        auto with typing.
-                      } {
-                        repeat constructor.
-                      }
+                  apply T_Apply with (Ty_Builtin (Some (TypeIn DefaultUniBool))). {
+                    apply T_TyInst with 
+                      (T1 := Ty_Fun (Ty_Builtin (Some (TypeIn DefaultUniBool))) (Ty_Fun (Ty_Var (TyName (Name "a" (Unique 0)))) (Ty_Fun (Ty_Var (TyName (Name "a" (Unique 0)))) (Ty_Var (TyName (Name "a" (Unique 0)))))))
+                      (X := "a")
+                      (K2 := Kind_Base)
+                      (T1' := (Ty_Fun (Ty_Builtin (Some (TypeIn DefaultUniBool)))
+                      (Ty_Fun (Ty_Var (TyName (Name "Bool" (Unique 11))))
+                          (Ty_Fun (Ty_Var (TyName (Name "Bool" (Unique 11))))
+                            (Ty_Var (TyName (Name "Bool" (Unique 11)))))))). {
+                      apply T_Builtin...
+                    }{
                       auto with typing.
+                    } {
+                      repeat constructor.
                     }
                     auto with typing.
                   }
@@ -733,166 +516,84 @@ Proof.
                 }
                 auto with typing.
               }
-              apply K_Builtin.
-            }
-            apply T_Apply with (Ty_Builtin (Some (TypeIn DefaultUniByteString))). {
-              apply T_Apply with (Ty_Builtin (Some (TypeIn DefaultUniByteString))). {
-                apply T_Builtin.
-              }
               auto with typing.
+            }
+            apply K_Builtin...
+          }
+          apply T_Apply with (Ty_Builtin (Some (TypeIn DefaultUniByteString))). {
+            apply T_Apply with (Ty_Builtin (Some (TypeIn DefaultUniByteString))). {
+              apply T_Builtin...
             }
             auto with typing.
           }
-          apply K_Builtin.
+          auto with typing.
         }
-        apply K_Builtin.
-    - auto with typing.
+        apply K_Builtin...
+      }
+      apply K_Builtin...
   }
-  simpl. eapply T_Let. {
-    reflexivity.
-  }{
-    apply W_ConsB_NonRec.
-    - apply W_Term.
-      + apply K_Builtin.
-      + apply T_Constant.
-    - auto with typing.
+  simpl. eapply T_Let... 
+  simpl. eapply T_Let...
+  simpl. eapply T_Let... {
+    apply W_ConsB_NonRec...
+    apply W_Term...
+    apply K_Fun...
   }
-  simpl. eapply T_Let. {
-    reflexivity.
-  }{
-    apply W_ConsB_NonRec.
-    - apply W_Term.
-      + apply K_Builtin.
-      + apply T_Constant.
-    - auto with typing.
+  simpl. eapply T_Let... {
+    apply W_ConsB_NonRec...
+    apply W_Term...
+    apply K_Fun...
   }
-  simpl. eapply T_Let. {
-    reflexivity.
-  }{
-    apply W_ConsB_NonRec.
-    - apply W_Term.
-      + apply K_Fun. {
-          apply K_Builtin.
-        } 
-        apply K_Fun. {
-          apply K_Builtin.
-        }
-        apply K_Builtin.
-      + apply T_Builtin.
-    - auto with typing.
+  simpl. eapply T_Let... {
+    apply W_ConsB_NonRec...
+    apply W_Term...
+    apply K_Fun...
   }
-  simpl. eapply T_Let. {
-    reflexivity.
-  }{
-    apply W_ConsB_NonRec.
-    - apply W_Term.
-      + apply K_Fun. {
-          apply K_Builtin.
-        } 
-        apply K_Fun. {
-          apply K_Builtin.
-        }
-        apply K_Builtin.
-      + apply T_Builtin.
-    - auto with typing.
+  simpl. eapply T_Let...
+  simpl. eapply T_Let... {
+    apply W_ConsB_NonRec...
+    apply W_Term...
   }
-  simpl. eapply T_Let. {
-    reflexivity.
-  }{
-    apply W_ConsB_NonRec.
-    - apply W_Term.
-      + apply K_Fun. {
-          apply K_Builtin.
-        } 
-        apply K_Fun. {
-          apply K_Builtin.
-        }
-        apply K_Builtin.
-      + apply T_Builtin.
-    - auto with typing.
+  simpl. eapply T_Let... {
+    apply W_ConsB_NonRec...
+    apply W_Term...
+    apply K_Fun...
   }
-  simpl. eapply T_Let. {
-    reflexivity.
-  }{
-    apply W_ConsB_NonRec.
-    - apply W_Type.
-      apply K_Builtin.
-    - auto with typing.
+  simpl. eapply T_Let... {
+    apply W_ConsB_NonRec...
+    apply W_Term...
+    apply K_Fun...
   }
-  simpl. eapply T_Let. {
-    reflexivity.
-  }{
-    apply W_ConsB_NonRec.
-    - apply W_Term.
-      + apply K_Fun. {
-          apply K_Builtin.
-        } 
-        apply K_Builtin.
-      + apply T_Builtin.
-    - auto with typing.
-  }
-  simpl. eapply T_Let. {
-    reflexivity.
-  }{
-    apply W_ConsB_NonRec.
-    - apply W_Term.
-      + apply K_Fun. {
-          apply K_Builtin.
-        } 
-        apply K_Fun. {
-          apply K_Builtin.
-        } 
-        apply K_Builtin.
-      + apply T_Builtin.
-    - auto with typing.
-  }
-  simpl. eapply T_Let. {
-    reflexivity.
-  }{
-    apply W_ConsB_NonRec.
-    - apply W_Term.
-      + apply K_Fun. {
-          apply K_Builtin.
-        } 
-        apply K_Fun. {
-          apply K_Builtin.
-        } 
-        apply K_Builtin.
-      + apply T_Builtin.
-    - auto with typing.
-  }
-  simpl. eapply T_Let. {
-    reflexivity.
-  }{
-    apply W_ConsB_NonRec.
-    - eapply W_Data.
-      + reflexivity.
-      + intros.
+  simpl. eapply T_Let... {
+    apply W_ConsB_NonRec...
+    eapply W_Data...
+    intros.
+    destruct H. {
+      subst.
+      eapply W_Con.
+      - simpl. eauto.
+      - intros.
         destruct H. {
           subst.
-          eapply W_Con.
-          - simpl. eauto.
-          - intros.
-            destruct H. {
-              subst.
-              apply K_Builtin.
-            }
-            destruct H.
-        }
-        destruct H. {
-          subst.
-          eapply W_Con.
-          - simpl. eauto.
-          - intros.
-            destruct H.
+          apply K_Builtin...
         }
         destruct H.
-    - auto with typing.
+      }
+      destruct H. {
+        subst.
+        eapply W_Con.
+        - simpl. eauto.
+        - intros.
+          destruct H.
+      }
+      destruct H.
   }
   apply T_LamAbs. {
     apply T_LamAbs. {
       eapply T_Let. {
         reflexivity.
+      }{
+        reflexivity. 
       }{
         apply W_ConsB_NonRec.
         - apply W_Term.
@@ -905,6 +606,8 @@ Proof.
       eapply T_Let. {
         reflexivity.
       }{
+        reflexivity.
+      } {
         apply W_ConsB_NonRec.
         - apply W_Term.
           + apply K_Var.
@@ -953,7 +656,7 @@ Proof.
             }
             auto with typing.
           }
-          apply K_Builtin.
+          apply K_Builtin...
         }
         apply T_LamAbs. {
           apply T_Var.
@@ -963,7 +666,7 @@ Proof.
       }
       auto with typing.
     }
-    apply K_Builtin.
+    apply K_Builtin...
   }
   auto with typing.
 Qed.
