src/Language/PlutusIR/Semantics/SemanticEquivalence/CompatibilityLemmas.v
@@ -7,6 +7,7 @@ Require Export PlutusCert.Language.PlutusIR.Semantics.SemanticEquivalence.Compat
 Require Export PlutusCert.Language.PlutusIR.Semantics.SemanticEquivalence.CompatibilityLemmas.IWrap.
 Require Export PlutusCert.Language.PlutusIR.Semantics.SemanticEquivalence.CompatibilityLemmas.LamAbs.
 Require Export PlutusCert.Language.PlutusIR.Semantics.SemanticEquivalence.CompatibilityLemmas.LetNonRec.
+Require Export PlutusCert.Language.PlutusIR.Semantics.SemanticEquivalence.CompatibilityLemmas.LetRec.
 Require Export PlutusCert.Language.PlutusIR.Semantics.SemanticEquivalence.CompatibilityLemmas.Unwrap.
 Require Export PlutusCert.Language.PlutusIR.Semantics.SemanticEquivalence.CompatibilityLemmas.TermBind.
 Require Export PlutusCert.Language.PlutusIR.Semantics.SemanticEquivalence.CompatibilityLemmas.TyAbs.
@@ -24,7 +25,9 @@ Create HintDb DSP_compatibility_lemmas.
   compatibility_ExtBuiltin
   compatibility_IWrap
   compatibility_LamAbs
-  compatibility_LetNonRec
+  compatibility_LetNonRec_nil
+  compatibility_LetNonRec_cons
+  compatibility_LetRec
   compatibility_TermBind
   compatibility_TyAbs
   compatibility_TyInst
@@ -32,9 +35,39 @@ Create HintDb DSP_compatibility_lemmas.
   compatibility_Unwrap
   compatibility_Var : DSP_compatibility_lemmas.
 
+Require Import Coq.Lists.List.
+Require Import PlutusCert.Language.PlutusIR.Semantics.Static.Implementations.
 
-Lemma distr_projection_application : forall {A B C D: Type} (f : A * B -> C * D) (p : A * B),
-    (fst (f p), snd (f p)) = f (fst p, snd p).
-Proof. destruct p. simpl. destruct f. simpl. reflexivity. Qed.
+Lemma flatten_app : forall {A B : Type} (f : A -> list B) (l : list A) x,
+    flatten (List.map f (x :: l)) = flatten (List.map f l) ++ f x.
+Proof.
+  intros.
+  unfold flatten.
+  simpl.
+  rewrite concat_app.
+  simpl.
+  rewrite app_nil_r.
+  reflexivity.
+Qed.
 
-#[export] Hint Resolve distr_projection_application : DSP_compatibility_lemmas.
+Require Import PlutusCert.Language.PlutusIR.Semantics.SemanticEquivalence.LogicalRelation.RelationalModel.
+
+Lemma helper : forall Delta Gamma b bs e e' T,
+    LR_logically_approximate 
+      (mupdate Delta (flatten (List.map binds_Delta (b :: bs)))) 
+      (mupdate Gamma (flatten (List.map binds_Gamma (b :: bs))))
+      e e' T ->
+    LR_logically_approximate
+      (mupdate (mupdate Delta (binds_Delta b)) (flatten (List.map binds_Delta bs)))
+      (mupdate (mupdate Gamma (binds_Gamma b)) (flatten (List.map binds_Gamma bs)))
+      e e' T.
+Proof.
+  intros.
+  rewrite <- mupdate_app.
+  rewrite <- mupdate_app.
+  rewrite <- flatten_app.
+  rewrite <- flatten_app.
+  assumption.
+Qed.
+
+#[export] Hint Resolve helper : DSP_compatibility_lemmas.
