src/Language/PlutusIR/Semantics/SemanticEquivalence/CompatibilityLemmas/LetNonRec.v
@@ -4,6 +4,8 @@ Require Import PlutusCert.Language.PlutusIR.Semantics.SemanticEquivalence.Logica
 Require Import PlutusCert.Language.PlutusIR.Semantics.SemanticEquivalence.Monotonicity.
 Require Import PlutusCert.Language.PlutusIR.Semantics.SemanticEquivalence.Auto.
 Require Import PlutusCert.Util.
+Require Import PlutusCert.Util.Map.
+Require Import PlutusCert.Util.Map.Mupdate.
 
 Require Import Arith.
 Require Import Coq.Lists.List.
@@ -205,40 +207,6 @@ Proof.
     + simpl. 
 Admitted.
 
-Inductive LR_logically_approximate_bindings_nonrec : Delta -> Gamma -> list Binding -> list Binding -> Prop :=
-  | LR_NonRec_Nil : forall Delta Gamma,
-      LR_logically_approximate_bindings_nonrec Delta Gamma nil nil
-  | LR_NonRec_Cons : forall Delta Gamma b b' Delta' Gamma' bs bs',
-      LR_logically_approximate_binding Delta Gamma b b' ->
-      (Delta', Gamma') = Implementations.append (binds b) (Delta, Gamma) ->
-      binds b = binds b' ->
-      LR_logically_approximate_bindings_nonrec Delta' Gamma' bs bs' ->
-      LR_logically_approximate_bindings_nonrec Delta Gamma (b :: bs) (b' :: bs').
-
-Lemma LR_la_bnr__oks : forall Delta Gamma bs bs',
-    LR_logically_approximate_bindings_nonrec Delta Gamma bs bs' ->
-    (Delta, Gamma) |-oks_nr bs /\ (Delta, Gamma) |-oks_nr bs' /\ List.map binds bs = List.map binds bs'.
-Proof.
-  intros.
-  induction H.
-  - eauto with typing.
-  - split.
-    + econstructor.
-      * apply H.
-      * rewrite <- H0.
-        apply IHLR_logically_approximate_bindings_nonrec.
-    + split. 
-      * econstructor.
-        -- apply H.
-        -- rewrite <- H1.
-          rewrite <- H0.
-          apply IHLR_logically_approximate_bindings_nonrec.
-      * simpl.
-        rewrite H1.
-        f_equal.
-        apply IHLR_logically_approximate_bindings_nonrec.
-Qed.
-
 Lemma msubst_term__fold : forall ss x v t,
     msubst_term ss <{ [v / x] t }> = msubst_term ((x, v) :: ss) t.
 Proof. induction ss; intros; auto. Qed.
@@ -247,180 +215,212 @@ Lemma msubst_bindings_nonrec__fold : forall ss x v bs,
     msubst_bindings_nonrec ss <{ [v / x][bnr] bs }> = msubst_bindings_nonrec ((x, v) :: ss) bs.
 Proof. induction ss; intros; auto. Qed.
 
-Lemma compatibility_LetNonRec : forall bs Delta Gamma t bs' t' T,
-    forall Delta' Gamma',
-      (Delta', Gamma') = append (flatten (List.map binds bs)) (Delta, Gamma) ->
-      LR_logically_approximate Delta' Gamma' t t' T ->
-      LR_logically_approximate_bindings_nonrec Delta Gamma bs bs' ->
-      LR_logically_approximate Delta Gamma (Let NonRec bs t) (Let NonRec bs' t') T.
+Lemma compatibility_LetNonRec_nil : forall Delta Gamma t t' T,
+    LR_logically_approximate Delta Gamma t t' T ->
+    LR_logically_approximate Delta Gamma (Let NonRec nil t) (Let NonRec nil t') T.
 Proof with eauto_LR.
-  induction bs.
-  - intros Delta Gamma t bs' t' T Delta' Gamma' Hbinds IH_LR__t IH_LR__bs.
-    unfold LR_logically_approximate.
+  intros Delta Gamma t t' T IHLR__t.
+  unfold LR_logically_approximate.
 
-    destruct IH_LR__t as [Htyp__t [Htyp__t' IH__t]].
-    inversion IH_LR__bs. subst.
+  destruct IHLR__t as [Htyp__t [Htyp__t' IH__t]].
 
-    split...
-    split...
+  split...
+  split...
 
-    intros k rho env env' ct ck HeqDelta HeqGamma H_RD H_RG.
+  intros k rho env env' ct ck HeqDelta HeqGamma H_RD H_RG.
+  subst.
+
+  autorewrite with RC.
+
+  split...
+  split...
+
+  rewrite msubstA_LetNonRec_nil. rewrite msubstA_LetNonRec_nil.
+  rewrite msubst_LetNonRec_nil. rewrite msubst_LetNonRec_nil.
+
+  intros j Hlt__j e_f Hev__e_f.
+
+  inversion Hev__e_f. subst.
+  inversion H3. subst.
+  rename j0 into j_1.
+  rename H3 into Hev'__e_f.
+  rename H0 into Hev''__e_f.
+  
+
+  assert (HRC__t : RC k T rho 
+    (msubst_term env (msubstA_term (msyn1 rho) t))
+    (msubst_term env' (msubstA_term (msyn2 rho) t'))
+  )...
+
+  apply RC_to_RV with (j := j_1) (e_f := e_f) in HRC__t as temp...
+  destruct temp as [e'_f1 [j'_1 [Hev__e'_f1 HRV__t]]].
+
+  eexists. eexists.
+
+  split. eapply E_Let. eapply E_NilB_NonRec...
+
+  eapply RV_condition... 
+  eapply RV_monotone...
+Qed.
+
+Lemma mupdate_flatten : forall {X : Type} (m : partial_map X) x l,
+    mupdate m (flatten (x :: l)) = mupdate (mupdate m x) (flatten l).
+Proof.
+  intros.
+  unfold flatten.
+  simpl.
+  rewrite concat_app.
+  simpl.
+  rewrite app_nil_r.
+  rewrite <- mupdate_app.
+  reflexivity.
+Qed.
+
+
+Lemma compatibility_LetNonRec_cons : forall Delta Gamma b bs t b' bs' t' T,
+    forall Delta_ih Gamma_ih,
+      Delta_ih = mupdate Delta (binds_Delta b) ->
+      Gamma_ih = mupdate Gamma (binds_Gamma b) ->
+      LR_logically_approximate Delta_ih Gamma_ih (Let NonRec bs t) (Let NonRec bs' t') T ->
+      LR_logically_approximate_binding Delta Gamma b b' ->
+      LR_logically_approximate Delta Gamma (Let NonRec (b :: bs) t) (Let NonRec (b' :: bs') t') T.
+Proof with eauto_LR.
+  intros Delta Gamma b bs t b' bs' t' T Delta_ih Gamma_ih Heq__Delta_ih Heq__Gamma_ih IHLR__ih IHLR__b.
+  subst.
+
+  destruct IHLR__ih as [Htyp__ih [Htyp__ih' IH__ih]].
+  destruct IHLR__b as [Htyp__b [Htyp__b' IH__b]].
+
+  inversion Htyp__ih. subst.
+  inversion Htyp__ih'. subst.
+
+  assert (Heq__bindsD : binds_Delta b = binds_Delta b'). {
+    destruct b, b'.
+    all: try solve [destruct v; destruct v0; auto].
+    all: try solve [destruct v; exfalso; auto].
+    all: try solve [inversion IH__b; auto].
+  }
+
+  assert (Heq__bindsG : binds_Gamma b = binds_Gamma b'). {
+    destruct b, b'.
+    all: try solve [destruct v; destruct v0; destruct IH__b as [Heq1 [Heq2 [Heq3 _]]]; subst; auto].
+    all: try solve [destruct v; exfalso; auto].
+    all: try solve [inversion IH__b; auto].
+  }
+
+  rewrite Heq__bindsD in H6.
+  rewrite Heq__bindsG in H6.
+  rewrite Heq__bindsD in H9.
+  rewrite Heq__bindsG in H9.
+
+  clear Heq__bindsD Heq__bindsG.
+
+  rewrite <- mupdate_flatten in H7.
+  rewrite <- mupdate_flatten in H7.
+  rewrite <- mupdate_flatten in H9.
+  rewrite <- mupdate_flatten in H9.
+
+  split...
+  split...
+
+  intros k rho env env' cG cD Heq__Delta Heq__Gamma HRD HRG.
+  subst.
+
+  autorewrite with RC.
+
+  split...
+  split...
+
+  clear H5 H7 H6 H9.
+  clear Htyp__ih Htyp__ih' Htyp__b Htyp__b'.
+
+  destruct b, b'.
+  - destruct v, v0.
+    
+    destruct IH__b as [Heq1 [Heq2 [Heq3 IHLR__tb]]].
     subst.
 
-    autorewrite with RC.
-
-    split...
-    split...
-
-    rewrite msubstA_LetNonRec_nil. rewrite msubstA_LetNonRec_nil.
-    rewrite msubst_LetNonRec_nil. rewrite msubst_LetNonRec_nil.
+    rename s1 into x.
+    rename t2 into Tb.
+    rename t0 into tb.
+    rename t1 into tb'.
+  
+    rewrite msubstA_LetNonRec. rewrite msubstA_LetNonRec.
+    rewrite msubstA_BindingsNonRec_cons. rewrite msubstA_BindingsNonRec_cons.
+    rewrite msubst_LetNonRec. rewrite msubst_LetNonRec.
+    rewrite msubst_BindingsNonRec_cons. rewrite msubst_BindingsNonRec_cons.
+    rewrite msubstA_TermBind. rewrite msubstA_TermBind.
+    rewrite msubst_TermBind. rewrite msubst_TermBind.
 
     intros j Hlt__j e_f Hev__e_f.
-
-    inversion Hev__e_f. subst.
-    inversion H3. subst.
-    rename j0 into j_1.
-    rename H3 into Hev'__e_f.
-    rename H0 into Hev''__e_f.
     
+    inversion Hev__e_f. subst.
+    clear Hev__e_f. rename H3 into Hev__e_f.
+    inversion Hev__e_f. subst.
+    clear Hev__e_f.
+    rename H7 into Hev__vb.
+    rename H8 into Hev__e_f.
 
-    assert (HRC__t : RC k T rho 
-      (msubst_term env (msubstA_term (msyn1 rho) t))
-      (msubst_term env' (msubstA_term (msyn2 rho) t'))
+    destruct IHLR__tb as [_ [_ IH__tb]].
+    assert (HRC__tb :
+      RC k Tb rho
+        (msubst_term env (msubstA_term (msyn1 rho) tb))
+        (msubst_term env' (msubstA_term (msyn2 rho) tb'))  
+    )...
+    clear IH__tb.
+
+    eapply RC_to_RV with (j := jb) (e_f := vb) in HRC__tb as temp...
+    destruct temp as [vb' [jb' [Hev__vb' HRV__vb]]].
+    clear Hev__vb.
+    clear HRC__tb.
+
+    assert (HRC__ih :
+      RC (k - jb -1) T rho
+        <{ /[ (x, vb) :: drop x env /] ( /[[ msyn1 rho /] {Let NonRec bs t} ) }>
+        <{ /[ (x, vb') :: drop x env' /] ( /[[ msyn2 rho /] {Let NonRec bs' t'} ) }>
     ). {
-      simpl in Hbinds. 
-      rewrite flatten_nil in Hbinds.
-      rewrite append_emptyContext_l in Hbinds.
-      inversion Hbinds. subst.
-      eapply IH__t...
+      apply IH__ih with (ct := (x, Tb) :: drop x cG) (ck := cD).
+      - reflexivity.
+      - apply mupdate_drop.
+      - assumption.
+      - assert (closed vb). {
+          eapply typable_empty__closed.
+          eapply RV_typable_empty_1...
+        }
+        assert (closed vb'). {
+          eapply typable_empty__closed.
+          eapply RV_typable_empty_2...
+        }
+        replace vb with (msubstA_term (msyn1 rho) vb) by (eapply msubstA_closed; eauto).
+        replace vb' with (msubstA_term (msyn2 rho) vb') by (eapply msubstA_closed; eauto).
+        apply RG_cons.
+        + apply RV_monotone with (k := k - jb)...
+          rewrite msubstA_closed...
+          rewrite msubstA_closed...
+        + apply RG_monotone with (k := k)...
+          apply RG_drop...
     }
+    clear IH__ih.
 
-    apply RC_to_RV with (j := j_1) (e_f := e_f) in HRC__t as temp...
-    destruct temp as [e'_f1 [j'_1 [Hev__e'_f1 HRV__t]]].
+    apply RC_to_RV with (j := j0) (e_f := e_f) in HRC__ih as temp...
+    * destruct temp as [e'_f [j0' [Hev__e'_f HRV0]]].
+      clear Hev__e_f.
 
-    eexists. eexists.
+      rewrite msubstA_LetNonRec in Hev__e'_f.
+      rewrite msubst_LetNonRec in Hev__e'_f.
 
-    split. eapply E_Let. eapply E_NilB_NonRec...
+      rewrite <- msubstA_bnr__bvbs in Hev__e'_f.
 
-    eapply RV_condition... 
-    eapply RV_monotone...
+      inversion Hev__e'_f. subst.
 
-  - intros Delta Gamma t bs' t' T Delta' Gamma' Hbinds IH_LR__t IH_LR__bbs.
-    unfold LR_logically_approximate.
-    rename a into b.
-
-    inversion IH_LR__bbs. subst.
-
-    rename bs'0 into bs'.
-    rename Delta'0 into Delta''.
-    rename Gamma'0 into Gamma''.
-    rename H1 into IH_LR__b.
-    rename H2 into Hbinds''.
-    rename H7 into IH_LR__bs.
-
-    assert (IH_LR__let : 
-      LR_logically_approximate Delta'' Gamma''
-        (Let NonRec bs t) (Let NonRec bs' t') T
-    ). {
-      eapply IHbs...
-      simpl in Hbinds.
-      unfold flatten in Hbinds.
-      simpl in Hbinds.
-      rewrite concat_append in Hbinds.
-      simpl in Hbinds.
-      rewrite append_emptyContext_r in Hbinds.
-      apply skip. (* TODO *)
-    }
-
-    destruct IH_LR__t as [Htyp__t [Htyp__t' IH__t]].
-    destruct IH_LR__b as [Htyp__b [Htyp__b' IH__b]].
-    eapply LR_la_bnr__oks in IH_LR__bbs.
-    destruct IH_LR__bbs as [Htyp__bbs [Htyp__bbs' Heqbinds__bbs]].
-
-    remember Hbinds as Hbinds'. clear HeqHbinds'.
-    rewrite Heqbinds__bbs in Hbinds'.
-
-    split...
-    split...
-
-    intros k rho env env' ct ck HeqDelta HeqGamma H_RD H_RG.
-    subst.
-
-    autorewrite with RC.
-
-    split...
-    split...
-
-    (* Some context management *)
-    clear IHbs.
-    clear Htyp__t.
-    clear Htyp__t'.
-    clear Htyp__bbs.
-    clear Htyp__bbs'.
-    clear Heqbinds__bbs.
-    clear Htyp__b.
-    clear Htyp__b'.
-    clear H5.
-    clear IH_LR__bs. 
-    clear IH__t.
-
-    destruct b, b'.
-    + destruct v. destruct v0.
-      rename s into s.
-      rename s0 into s'.
-      rename s1 into x.
-      rename s2 into x'.
-      rename t2 into Tb.
-      rename t3 into Tb'.
-      rename t0 into tb.
-      rename t1 into tb'.
-
-      destruct IH__b as [Heq1 [Heq2 [Heq3 IH_LR__tb]]].
-      subst.
-
-      rewrite msubstA_LetNonRec. rewrite msubstA_LetNonRec.
-      rewrite msubstA_BindingsNonRec_cons. rewrite msubstA_BindingsNonRec_cons.
-      rewrite msubst_LetNonRec. rewrite msubst_LetNonRec.
-      rewrite msubst_BindingsNonRec_cons. rewrite msubst_BindingsNonRec_cons.
-      rewrite msubstA_TermBind. rewrite msubstA_TermBind.
-      rewrite msubst_TermBind. rewrite msubst_TermBind.
-
-      intros j Hlt__j e_f Hev__e_f.
-      inversion Hev__e_f. subst.
-      clear Hev__e_f. rename H3 into Hev__e_f.
-      inversion Hev__e_f. subst.
-      rename H7 into Hev__vb.
-      rename H8 into Hev'__e_f.
-
-      destruct IH_LR__tb as [_ [_ IH__tb]].
-      assert (HRC__tb :
-        RC k Tb rho
-          (msubst_term env (msubstA_term (msyn1 rho) tb))
-          (msubst_term env' (msubstA_term (msyn2 rho) tb'))  
-      )...
-
-      eapply RC_to_RV with (j := jb) (e_f := vb) in HRC__tb as temp...
-      destruct temp as [vb' [jb' [Hev__vb' HRV__vb]]].
-      clear Hev__vb.
-
-      destruct IH_LR__let as [_ [_ IH__let]].
-
-      assert (HRC__let :
-        RC (k - jb -1) T rho
-          <{ /[ (x, vb) :: drop x env /] ( /[[ msyn1 rho /] {Let NonRec bs t} ) }>
-          <{ /[ (x, vb') :: drop x env' /] ( /[[ msyn2 rho /] {Let NonRec bs' t'} ) }>
-      ). {
-        apply IH__let with (ct := (x, Tb) :: drop x ct) (ck := ck).
-        - simpl in Hbinds''.
-          rewrite append_singleton_l in Hbinds''.
-          inversion Hbinds''. subst.
-          reflexivity.
-        - simpl in Hbinds''.
-          rewrite append_singleton_l in Hbinds''.
-          inversion Hbinds''. subst.
-          simpl.
-          apply mupdate_drop.
-        - assumption.
+      eexists. eexists.
+      split. {
+        apply E_Let.
+        apply E_ConsB_NonRec with (vb := vb') (jb := jb') (v := e'_f) (j := j0')...
+        simpl.
+        rewrite <- msubst_bnr__bound_vars.
+        rewrite <- msubstA_bnr__bvbs.
+        destruct (existsb (eqb x) (bvbs bs')) eqn:Hexb.
         - assert (closed vb). {
             eapply typable_empty__closed.
             eapply RV_typable_empty_1...
@@ -429,128 +429,19 @@ Proof with eauto_LR.
             eapply typable_empty__closed.
             eapply RV_typable_empty_2...
           }
-          replace vb with (msubstA_term (msyn1 rho) vb) by (eapply msubstA_closed; eauto).
-          replace vb' with (msubstA_term (msyn2 rho) vb') by (eapply msubstA_closed; eauto).
-          apply RG_cons.
-          + apply RV_monotone with (k := k - jb)...
-            rewrite msubstA_closed...
-            rewrite msubstA_closed...
-          + apply RG_monotone with (k := k)...
-            apply RG_drop...
-      }
-
-      apply RC_to_RV with (j := j0) (e_f := e_f) in HRC__let as temp...
-      * destruct temp as [e'_f [j0' [Hev__e'_f HRV0]]].
-
-        rewrite msubstA_LetNonRec in Hev__e'_f.
-        rewrite msubst_LetNonRec in Hev__e'_f.
-
-        rewrite <- msubstA_bnr__bvbs in Hev__e'_f.
-
-        inversion Hev__e'_f. subst.
-
-        eexists. eexists.
-        split. {
-          apply E_Let.
-          apply E_ConsB_NonRec with (vb := vb') (jb := jb') (v := e'_f) (j := j0')...
-          simpl.
-          rewrite <- msubst_bnr__bound_vars.
-          rewrite <- msubstA_bnr__bvbs.
-          destruct (existsb (eqb x) (bvbs bs')) eqn:Hexb.
-          - assert (closed vb). {
-              eapply typable_empty__closed.
-              eapply RV_typable_empty_1...
-            }
-            assert (closed vb'). {
-              eapply typable_empty__closed.
-              eapply RV_typable_empty_2...
-            }
-            apply RG_env_closed in H_RG as Hclss.
-            destruct Hclss as [Hcls__env Hcls__env'].
-            rewrite <- subst_bnr__msubst_bnr'...
-            replace (concat (map bvb <{ /[[ msyn2 rho /][bnr] bs' }>)) with
-              (bvbs  <{ /[[ msyn2 rho /][bnr] bs' }>)...
-            rewrite <- msubstA_bnr__bvbs.
-
-            apply existsb_exists in Hexb.
-            destruct Hexb as [y [HIn Heqb]].
-            apply eqb_eq in Heqb as Heq.
-            subst.
-            rewrite In__mdrop in H3...
-          - assert (closed vb). {
-              eapply typable_empty__closed.
-              eapply RV_typable_empty_1...
-            }
-            assert (closed vb'). {
-              eapply typable_empty__closed.
-              eapply RV_typable_empty_2...
-            }
-            apply RG_env_closed in H_RG as Hclss.
-            destruct Hclss as [Hcls__env Hcls__env'].
-            rewrite <- subst_bnr__msubst_bnr'...
-            replace (concat (map bvb <{ /[[ msyn2 rho /][bnr] bs' }>)) with
-              (bvbs  <{ /[[ msyn2 rho /][bnr] bs' }>)...
-            rewrite <- msubstA_bnr__bvbs.
-
-            apply existsb_nexists in Hexb.
-            rewrite not_In__mdrop in H3...
-            + unfold btvbs. simpl.
-              replace (concat (map btvb bs')) with (btvbs bs')...
-
-              rewrite <- subst_msubst''...
-              * eapply RG_env_closed.
-                eapply RG_drop...
-              * intros Hcon.
-                apply Hexb.
-                exists x.
-                rewrite eqb_refl.
-                eauto.
-            + intros Hcon.
-              apply Hexb.
-              exists x.
-              rewrite eqb_refl.
-              eauto.
-        }
-
-        eapply RV_condition...
-        replace (k - (jb + 1 + j0)) with (k - jb - 1 - j0)...
-      * rewrite msubstA_LetNonRec.
-        rewrite msubst_LetNonRec. 
-        apply E_Let.
-
-        simpl.
-        simpl in Hev'__e_f.
-
-        rewrite <- msubst_bnr__bound_vars in Hev'__e_f.
-        rewrite <- msubstA_bnr__bvbs in Hev'__e_f.
-
-        destruct (existsb (eqb x) (bvbs bs)) eqn:Hexb. {
-          assert (closed vb). {
-            eapply typable_empty__closed.
-            eapply RV_typable_empty_1...
-          }
-          assert (closed vb'). {
-            eapply typable_empty__closed.
-            eapply RV_typable_empty_2...
-          }
-          apply RG_env_closed in H_RG as Hclss.
+          apply RG_env_closed in HRG as Hclss.
           destruct Hclss as [Hcls__env Hcls__env'].
-          rewrite <- subst_bnr__msubst_bnr' in Hev'__e_f...
-          replace (concat (map bvb <{ /[[ msyn1 rho /][bnr] bs }>)) with
-            (bvbs <{ /[[ msyn1 rho /][bnr] bs }>) in Hev'__e_f...
-          
-          unfold btvbs in Hev'__e_f.
-          simpl in Hev'__e_f.
+          rewrite <- subst_bnr__msubst_bnr'...
+          replace (concat (map bvb <{ /[[ msyn2 rho /][bnr] bs' }>)) with
+            (bvbs  <{ /[[ msyn2 rho /][bnr] bs' }>)...
           rewrite <- msubstA_bnr__bvbs.
-          rewrite <- msubstA_bnr__bvbs in Hev'__e_f.
 
           apply existsb_exists in Hexb.
           destruct Hexb as [y [HIn Heqb]].
           apply eqb_eq in Heqb as Heq.
           subst.
-          rewrite In__mdrop...
-        } {
-          assert (closed vb). {
+          rewrite In__mdrop in H3...
+        - assert (closed vb). {
             eapply typable_empty__closed.
             eapply RV_typable_empty_1...
           }
@@ -558,36 +449,109 @@ Proof with eauto_LR.
             eapply typable_empty__closed.
             eapply RV_typable_empty_2...
           }
-          apply RG_env_closed in H_RG as Hclss.
+          apply RG_env_closed in HRG as Hclss.
           destruct Hclss as [Hcls__env Hcls__env'].
-          rewrite <- subst_bnr__msubst_bnr' in Hev'__e_f...
-          replace (concat (map bvb <{ /[[ msyn1 rho /][bnr] bs }>)) with
-            (bvbs <{ /[[ msyn1 rho /][bnr] bs }>) in Hev'__e_f...
-          
-          unfold btvbs in Hev'__e_f.
-          simpl in Hev'__e_f.
+          rewrite <- subst_bnr__msubst_bnr'...
+          replace (concat (map bvb <{ /[[ msyn2 rho /][bnr] bs' }>)) with
+            (bvbs  <{ /[[ msyn2 rho /][bnr] bs' }>)...
           rewrite <- msubstA_bnr__bvbs.
-          rewrite <- msubstA_bnr__bvbs in Hev'__e_f.
 
           apply existsb_nexists in Hexb.
-          rewrite not_In__mdrop.
-          - replace (concat (map btvb bs)) with (btvbs bs) in Hev'__e_f...
-            rewrite <- subst_msubst'' in Hev'__e_f...
-            + eapply RG_env_closed_1.
+          rewrite not_In__mdrop in H3...
+          + unfold btvbs. simpl.
+            replace (concat (map btvb bs')) with (btvbs bs')...
+
+            rewrite <- subst_msubst''...
+            * eapply RG_env_closed.
               eapply RG_drop...
-            + intros Hcon.
+            * intros Hcon.
               apply Hexb.
               exists x.
               rewrite eqb_refl.
               eauto.
-          - intros Hcon.
+          + intros Hcon.
             apply Hexb.
             exists x.
             rewrite eqb_refl.
             eauto.
+      }
+
+      eapply RV_condition...
+      replace (k - (jb + 1 + j0)) with (k - jb - 1 - j0)...
+    * rewrite msubstA_LetNonRec.
+      rewrite msubst_LetNonRec. 
+      apply E_Let.
+
+      simpl.
+      simpl in Hev__e_f.
+
+      rewrite <- msubst_bnr__bound_vars in Hev__e_f.
+      rewrite <- msubstA_bnr__bvbs in Hev__e_f.
+
+      destruct (existsb (eqb x) (bvbs bs)) eqn:Hexb. {
+        assert (closed vb). {
+          eapply typable_empty__closed.
+          eapply RV_typable_empty_1...
         }
-  + destruct v. exfalso. auto.
-  + destruct v. exfalso. auto.
-  + exfalso. auto.
-  + 
+        assert (closed vb'). {
+          eapply typable_empty__closed.
+          eapply RV_typable_empty_2...
+        }
+        apply RG_env_closed in HRG as Hclss.
+        destruct Hclss as [Hcls__env Hcls__env'].
+        rewrite <- subst_bnr__msubst_bnr' in Hev__e_f...
+        replace (concat (map bvb <{ /[[ msyn1 rho /][bnr] bs }>)) with
+          (bvbs <{ /[[ msyn1 rho /][bnr] bs }>) in Hev__e_f...
+        
+        unfold btvbs in Hev__e_f.
+        simpl in Hev__e_f.
+        rewrite <- msubstA_bnr__bvbs.
+        rewrite <- msubstA_bnr__bvbs in Hev__e_f.
+
+        apply existsb_exists in Hexb.
+        destruct Hexb as [y [HIn Heqb]].
+        apply eqb_eq in Heqb as Heq.
+        subst.
+        rewrite In__mdrop...
+      } {
+        assert (closed vb). {
+          eapply typable_empty__closed.
+          eapply RV_typable_empty_1...
+        }
+        assert (closed vb'). {
+          eapply typable_empty__closed.
+          eapply RV_typable_empty_2...
+        }
+        apply RG_env_closed in HRG as Hclss.
+        destruct Hclss as [Hcls__env Hcls__env'].
+        rewrite <- subst_bnr__msubst_bnr' in Hev__e_f...
+        replace (concat (map bvb <{ /[[ msyn1 rho /][bnr] bs }>)) with
+          (bvbs <{ /[[ msyn1 rho /][bnr] bs }>) in Hev__e_f...
+        
+        unfold btvbs in Hev__e_f.
+        simpl in Hev__e_f.
+        rewrite <- msubstA_bnr__bvbs.
+        rewrite <- msubstA_bnr__bvbs in Hev__e_f.
+
+        apply existsb_nexists in Hexb.
+        rewrite not_In__mdrop.
+        - replace (concat (map btvb bs)) with (btvbs bs) in Hev__e_f...
+          rewrite <- subst_msubst'' in Hev__e_f...
+          + eapply RG_env_closed_1.
+            eapply RG_drop...
+          + intros Hcon.
+            apply Hexb.
+            exists x.
+            rewrite eqb_refl.
+            eauto.
+        - intros Hcon.
+          apply Hexb.
+          exists x.
+          rewrite eqb_refl.
+          eauto.
+      }
+  - destruct v. exfalso. auto.
+  - destruct v. exfalso. auto.
+  - exfalso. auto.
+  - 
 Admitted.
