src/Language/PlutusIR/Semantics/SemanticEquivalence/CompatibilityLemmas/LetRec.v
@@ -3,12 +3,6 @@ Require Import PlutusCert.Language.PlutusIR.Semantics.Static.
 Require Import PlutusCert.Language.PlutusIR.Semantics.SemanticEquivalence.LogicalRelation.RelationalModel.
 Require Import PlutusCert.Language.PlutusIR.Semantics.SemanticEquivalence.Auto.
 
-Lemma compatibility_DatatypeBind : forall Delta Gamma d,
-    Delta ,, Gamma |-ok (DatatypeBind d) ->
-    LR_logically_approximate_binding Delta Gamma (DatatypeBind d) (DatatypeBind d).
-Proof with eauto_LR.
-  intros Delta Gamma d Hok.
-  unfold LR_logically_approximate_binding.
-
-  split...
-Qed.
+Lemma compatibility_LetRec : forall Delta Gamma bs t bs' t' T,
+    LR_logically_approximate Delta Gamma (Let Rec bs t) (Let Rec bs' t') T.
+Proof with eauto_LR. Admitted.
