src/Language/PlutusIR/Semantics/Static.v
@@ -1,5 +1,4 @@
 (** The static semantics *)
-Require Export PlutusCert.Language.PlutusIR.Semantics.Static.Map.
 Require Export PlutusCert.Language.PlutusIR.Semantics.Static.Implementations.
 Require Export PlutusCert.Language.PlutusIR.Semantics.Static.Rules.
 Require Export PlutusCert.Language.PlutusIR.Semantics.Static.TypeSubstitution.
