src/Util/Map/Mupdate.v
@@ -1,0 +1,53 @@
+Require Import PlutusCert.Util.Map.
+
+Require Import Coq.Lists.List.
+Import ListNotations.
+Require Import Coq.Strings.String.
+Local Open Scope string_scope.
+
+Fixpoint mupdate {X:Type} (m : partial_map X) (xts : list (string * X)) :=
+  match xts with
+  | nil => m
+  | ((x, v) :: xts') => x |-> v ; (mupdate m xts')
+  end.
+
+Lemma mupdate_eq_cong : forall {X : Type} (m : @partial_map X) m' xts x,
+    m x = m' x ->
+    mupdate m xts x = mupdate m' xts x.
+Proof.
+  induction xts.
+  - intros. assumption.
+  - intros. simpl.
+    destruct a.
+    destruct (x =? s) eqn:Heqb.
+    + apply eqb_eq in Heqb as Heq.
+      subst.
+      rewrite update_eq.
+      rewrite update_eq.
+      auto.
+    + apply eqb_neq in Heqb.
+      rewrite update_neq; auto.
+      rewrite update_neq; auto.
+Qed.
+
+Lemma mupdate_app: forall {X : Type} (m : partial_map X) (l l' : list (string * X)),
+    mupdate m (l ++ l') = mupdate (mupdate m l') l.
+Proof.
+  induction l; intros.
+  - reflexivity.
+  - destruct a. simpl. f_equal. auto.
+Qed.
+    
+
+Lemma inclusion_mupdate : forall {X : Type} (m m' : partial_map X) xts,
+  inclusion m m' ->
+  inclusion (mupdate m xts) (mupdate m' xts).
+Proof.
+  induction xts.
+  - intros. assumption.
+  - intros. simpl.
+    destruct a.
+    apply inclusion_update.
+    auto.
+Qed.
+
